@prefix : <http://www.semanticweb.org/musicOntology#> .
@prefix owl: <http://www.w3.org/2002/07/owl#> .
@prefix rdf: <http://www.w3.org/1999/02/22-rdf-syntax-ns#> .
@prefix xml: <http://www.w3.org/XML/1998/namespace> .
@prefix xsd: <http://www.w3.org/2001/XMLSchema#> .
@prefix rdfs: <http://www.w3.org/2000/01/rdf-schema#> .
@base <http://www.semanticweb.org/musicOntology> .

<http://www.semanticweb.org/musicOntology> rdf:type owl:Ontology .


#################################################################
#
#    Object Properties
#
#################################################################


###  http://www.semanticweb.org/musicOntology#collectiveRole

:collectiveRole rdf:type owl:ObjectProperty ,
                         owl:TransitiveProperty ;
                
                rdfs:domain :CollectiveMember ;
                
                rdfs:range :CollectiveRole .



###  http://www.semanticweb.org/musicOntology#composer

:composer rdf:type owl:ObjectProperty ,
                   owl:TransitiveProperty ;
          
          rdfs:domain :MusicalComposition ;
          
          rdfs:range :Musician ,
                     :Performer ;
          
          owl:inverseOf :composer_of .



###  http://www.semanticweb.org/musicOntology#composer_of

:composer_of rdf:type owl:ObjectProperty ,
                      owl:TransitiveProperty ;
             
             rdfs:range :MusicalComposition ;
             
             rdfs:domain :Musician ,
                         :Performer .



###  http://www.semanticweb.org/musicOntology#from_album

:from_album rdf:type owl:ObjectProperty ;
            
            rdfs:range :Album ;
            
            rdfs:domain :Song ;
            
            owl:inverseOf :has_song .



###  http://www.semanticweb.org/musicOntology#has_album

:has_album rdf:type owl:ObjectProperty ,
                    owl:TransitiveProperty ;
           
           rdfs:range :Album ;
           
           rdfs:domain :Performer .



###  http://www.semanticweb.org/musicOntology#has_genre

:has_genre rdf:type owl:ObjectProperty ,
                    owl:TransitiveProperty ;
           
           rdfs:range :Genre ;
           
           rdfs:domain :Performer .



###  http://www.semanticweb.org/musicOntology#has_member

:has_member rdf:type owl:ObjectProperty ;
            
            rdfs:domain :Collective ;
            
            rdfs:range :CollectiveMember .



###  http://www.semanticweb.org/musicOntology#has_song

:has_song rdf:type owl:ObjectProperty ,
                   owl:TransitiveProperty ;
          
          rdfs:domain :Album ;
          
          rdfs:range :Song .



###  http://www.semanticweb.org/musicOntology#musician

:musician rdf:type owl:ObjectProperty ;
          
          rdfs:domain :CollectiveMember ;
          
          rdfs:range :Musician ;
          
          rdfs:domain :SoloPerformer .



###  http://www.semanticweb.org/musicOntology#performer

:performer rdf:type owl:ObjectProperty ,
                    owl:TransitiveProperty ;
           
           rdfs:domain :Album ,
                       :MusicalComposition ;
           
           rdfs:range :Performer .



###  http://www.semanticweb.org/musicOntology#performs

:performs rdf:type owl:ObjectProperty ,
                   owl:TransitiveProperty ;
          
          rdfs:range :MusicalComposition ;
          
          rdfs:domain :Performer ;
          
          owl:inverseOf :performer .



###  http://www.semanticweb.org/musicOntology#plays_on

:plays_on rdf:type owl:ObjectProperty ,
                   owl:TransitiveProperty ;
          
          rdfs:range :MusicalInstrument ;
          
          rdfs:domain :Musician .



###  http://www.semanticweb.org/musicOntology#primaryMusicalInstrument

:primaryMusicalInstrument rdf:type owl:ObjectProperty ,
                                   owl:TransitiveProperty ;
                          
                          rdfs:range :MusicalInstrument ;
                          
                          rdfs:domain :Musician .



###  http://www.semanticweb.org/musicOntology#recorded_on

:recorded_on rdf:type owl:ObjectProperty ,
                      owl:TransitiveProperty ;
             
             rdfs:domain :Album ;
             
             rdfs:range :Medium ;
             
             rdfs:domain :MusicalComposition .



###  http://www.w3.org/2002/07/owl#topObjectProperty

owl:topObjectProperty rdf:type owl:TransitiveProperty .





#################################################################
#
#    Data properties
#
#################################################################


###  http://www.semanticweb.org/musicOntology#name

:name rdf:type owl:DatatypeProperty ,
               owl:FunctionalProperty ;
      
      rdfs:domain :Album ,
                  :Medium ,
                  :Musician ,
                  :Performer ;
      
      rdfs:range xsd:string .





#################################################################
#
#    Classes
#
#################################################################


###  http://www.semanticweb.org/musicOntology#Aerophone

:Aerophone rdf:type owl:Class ;
           
           rdfs:label "Aerophone" ;
           
           rdfs:subClassOf :MusicalInstrument ;
           
           rdfs:comment "musical instruments, which are wood, metal and other tubes with various devices and forms, emits a musical sounds as a result of fluctuations in them prisoner air column." .



###  http://www.semanticweb.org/musicOntology#African

:African rdf:type owl:Class ;
         
         rdfs:label "African" ;
         
         rdfs:subClassOf :Genre ;
         
         rdfs:comment "African popular music, like African traditional music, is vast and varied. Most contemporary genres of African popular music build on cross-pollination with western popular music." .



###  http://www.semanticweb.org/musicOntology#Album

:Album rdf:type owl:Class ;
       
       rdfs:label "Album" ;
       
       rdfs:comment "An album is a recording originally issued in gramophone format, followed by the vinyl format, and has then been issued in other formats such as Compact Cassette, Compact disc, and increasingly in digital formats such as MP3, AAC, ALAC, or FLAC. Audio albums in physical form are often provided with decorative covers (cover art) and liner notes and inserts about the music and recording, giving background information and analysis of the recording, lyrics and librettos, images of the performers, and other images and text, as well as thanking contributors. When supplied with compact discs they are known as CD booklets." .



###  http://www.semanticweb.org/musicOntology#Asian

:Asian rdf:type owl:Class ;
       
       rdfs:label "Asian" ;
       
       rdfs:subClassOf :Genre ;
       
       rdfs:comment "Asian music encompasses numerous different musical styles originating from a large number of Asian countries." .



###  http://www.semanticweb.org/musicOntology#Avant-garde

:Avant-garde rdf:type owl:Class ;
             
             rdfs:label "Avant-garde" ;
             
             rdfs:subClassOf :Genre ;
             
             rdfs:comment "The term avant-garde is applied to music when it is considered \"ahead of its time\" by critics or fans, i.e., it contains unique or original elements, or it explores unusual fusions of different genres." .



###  http://www.semanticweb.org/musicOntology#BallroomDance

:BallroomDance rdf:type owl:Class ;
               
               rdfs:label "Ballroom dance" ;
               
               rdfs:subClassOf :Genre ;
               
               rdfs:comment "Ballroom dance is a set of partner dances, which are enjoyed both socially and competitively around the world, and growing all the more popular in North America. Because of its performance and entertainment aspects, ballroom dance is also widely enjoyed on stage, film, and television." .



###  http://www.semanticweb.org/musicOntology#Blues

:Blues rdf:type owl:Class ;
       
       rdfs:label "Blues" ;
       
       rdfs:subClassOf :Genre ;
       
       rdfs:comment "Blues is a genre and musical form that originated in African-American communities in the \"Deep South\" of the United States around the end of the 19th century. The genre is a fusion of traditional African music and European folk music, spirituals, work songs, field hollers, shouts and chants, and rhymed simple narrative ballads. The blues form, ubiquitous in jazz, rhythm and blues and rock and roll, is characterized by the call-and-response pattern and specific chord progressions, of which the twelve-bar blues is the most common. The blue notes are also an important part of the sound. Blues shuffles or walking bass reinforce the trance-like rhythm and form a repetitive effect called a groove" .



###  http://www.semanticweb.org/musicOntology#Brazilian

:Brazilian rdf:type owl:Class ;
           
           rdfs:label "Brazilian" ;
           
           rdfs:subClassOf :Latin ;
           
           rdfs:comment "The music of Brazil encompasses various regional music styles influenced by African, European and Amerindian forms. After 500 years of history, Brazilian music developed some unique and original styles such as samba, bossa nova, MPB, sertanejo, pagode, tropicalia, choro, maracatu, embolada (coco de repente), Mangue Bit, funk carioca (in Brazil simply known as Funk), frevo, forró, axé, brega, lambada, and Brazilian versions of foreign musical genres, such as Brazilian rock and rap." .



###  http://www.semanticweb.org/musicOntology#Caribbean-and-Caribbean-influenced

:Caribbean-and-Caribbean-influenced rdf:type owl:Class ;
                                    
                                    rdfs:label "Caribbean and Caribbean-influenced" ;
                                    
                                    rdfs:subClassOf :Genre ;
                                    
                                    rdfs:comment "Caribbean music genres are diverse. They are each syntheses of African, European, Indian and Indigenous influences, largely created by descendants of African slaves (see Afro-Caribbean music), along with contributions from other communities (such as Indo-Caribbean music). Some of the styles to gain wide popularity outside of the Caribbean include bouyon, cadence-lypso, calypso, compas, Jing ping, punta, reggae, reggaeton, soca, and zouk. Caribbean is also related to Central American and South American music." .



###  http://www.semanticweb.org/musicOntology#Chordophone

:Chordophone rdf:type owl:Class ;
             
             rdfs:label "Chordophone" ;
             
             rdfs:subClassOf :MusicalInstrument ;
             
             rdfs:comment "is a musical instrument in which the sound source (vibrator) are the vibration of the strings." .



###  http://www.semanticweb.org/musicOntology#Collective

:Collective rdf:type owl:Class ;
            
            rdfs:label "Collective" ;
            
            rdfs:subClassOf [ rdf:type owl:Class ;
                              owl:intersectionOf ( :Performer
                                                   [ rdf:type owl:Restriction ;
                                                     owl:onProperty :has_member ;
                                                     owl:onClass :CollectiveMember ;
                                                     owl:minQualifiedCardinality "2"^^xsd:nonNegativeInteger
                                                   ]
                                                 )
                            ] ;
            
            owl:disjointWith :SoloPerformer .



###  http://www.semanticweb.org/musicOntology#CollectiveMember

:CollectiveMember rdf:type owl:Class ;
                  
                  rdfs:label "Collective member" ;
                  
                  rdfs:subClassOf [ rdf:type owl:Class ;
                                    owl:intersectionOf ( :Performer
                                                         [ rdf:type owl:Restriction ;
                                                           owl:onProperty :collectiveRole ;
                                                           owl:onClass :CollectiveRole ;
                                                           owl:minQualifiedCardinality "1"^^xsd:nonNegativeInteger
                                                         ]
                                                         [ rdf:type owl:Restriction ;
                                                           owl:onProperty :musician ;
                                                           owl:onClass :Musician ;
                                                           owl:qualifiedCardinality "1"^^xsd:nonNegativeInteger
                                                         ]
                                                       )
                                  ] .



###  http://www.semanticweb.org/musicOntology#CollectiveRole

:CollectiveRole rdf:type owl:Class ;
                
                rdfs:label "Collective role" .



###  http://www.semanticweb.org/musicOntology#Comedy

:Comedy rdf:type owl:Class ;
        
        rdfs:label "Comedy" ;
        
        rdfs:subClassOf :Genre ;
        
        rdfs:comment "Comedy music is music that is comic or humorous in nature, encompassing a wide variety of music genres. Popular types of comedy music include parody music, novelty songs, comedy rock and comedy hip hop." .



###  http://www.semanticweb.org/musicOntology#Country

:Country rdf:type owl:Class ;
         
         rdfs:label "Country" ;
         
         rdfs:subClassOf :Genre ;
         
         rdfs:comment "Country music is a genre of American popular music that originated in Southern United States, in Atlanta, Georgia in the 1920s. It takes its roots from the southeastern genre of American folk music and Western music. Blues modes have been used extensively throughout its recorded history. Country music often consists of ballads and dance tunes with generally simple forms and harmonies accompanied by mostly string instruments such as banjos, electric and acoustic guitars, fiddles, and harmonicas." .



###  http://www.semanticweb.org/musicOntology#Duet

:Duet rdf:type owl:Class ;
      
      rdfs:label "Duet" ;
      
      rdfs:subClassOf [ rdf:type owl:Class ;
                        owl:intersectionOf ( :Collective
                                             [ rdf:type owl:Restriction ;
                                               owl:onProperty :has_member ;
                                               owl:onClass :CollectiveMember ;
                                               owl:qualifiedCardinality "2"^^xsd:nonNegativeInteger
                                             ]
                                           )
                      ] ;
      
      rdfs:comment "A duet is a musical composition for two performers in which the performers have equal importance to the piece. It is often used to describe a composition involving two singers. It differs from a harmony, as the performers take turns performing a solo section rather than performing simultaneously. In classical music, the term is most often used for a composition for two singers or pianists. A piece performed by two pianists performing together on the same piano is referred to as \"piano duet\" or \"piano four hands\". A piece for two pianists performing together on separate pianos is referred to as a \"piano duo\"." .



###  http://www.semanticweb.org/musicOntology#EastAsian

:EastAsian rdf:type owl:Class ;
           
           rdfs:label "East Asian" ;
           
           rdfs:subClassOf :Asian ;
           
           owl:disjointWith :South-and-southeastAsian .



###  http://www.semanticweb.org/musicOntology#Easy-listening

:Easy-listening rdf:type owl:Class ;
                
                rdfs:label "Easy listening" ;
                
                rdfs:subClassOf :Genre ;
                
                rdfs:comment "Easy listening (also known as orchestral pop) is a popular music genre and radio format that was most popular during the 1950s to 1970s. It is related to middle-of-the-road (MOR) music and encompasses instrumental recordings of standards, hit songs and popular non-rock vocals. It was differentiated from the mostly instrumental beautiful music format by its variety of styles, including a percentage of vocals, arrangements and tempos to fit various day parts during the broadcast day." .



###  http://www.semanticweb.org/musicOntology#Electronic

:Electronic rdf:type owl:Class ;
            
            rdfs:label "Electronic" ;
            
            rdfs:subClassOf :Genre ;
            
            rdfs:comment "Electronic music is music that employs electronic musical instruments and electronic music technology in its production, an electronic musician being a musician who composes and/or performs such music. In general a distinction can be made between sound produced using electromechanical means and that produced using electronic technology. Examples of electromechanical sound producing devices include the telharmonium, Hammond organ, and the electric guitar. Purely electronic sound production can be achieved using devices such as the theremin, sound synthesizer, and computer." .



###  http://www.semanticweb.org/musicOntology#Electrophone

:Electrophone rdf:type owl:Class ;
              
              rdfs:label "Electrophone" ;
              
              rdfs:subClassOf :MusicalInstrument ;
              
              rdfs:comment "musical instruments, are used to generate (including fusion) sound different electronic circuits. Such tools can create sound by varying the volume, frequency, or duration of each segment generated." .



###  http://www.semanticweb.org/musicOntology#Ensemble

:Ensemble rdf:type owl:Class ;
          
          rdfs:label "Ensemble" ;
          
          rdfs:subClassOf [ rdf:type owl:Class ;
                            owl:intersectionOf ( :Collective
                                                 [ rdf:type owl:Restriction ;
                                                   owl:onProperty :has_member ;
                                                   owl:onClass :CollectiveMember ;
                                                   owl:minQualifiedCardinality "9"^^xsd:nonNegativeInteger
                                                 ]
                                               )
                          ] ;
          
          rdfs:comment "A musical ensemble, also known as a music group, is a group of people who perform instrumental or vocal music, typically known by a distinct name. In classical music, trios or quartets either blend the sounds of musical instrument families (such as piano, strings, and wind instruments) or group together instruments from the same instrument family, such as string ensembles or wind ensembles. In jazz ensembles, the instruments typically include wind instruments (one or more saxophones, trumpets, etc.), one or two chordal \"comping\" instruments (electric guitar, piano, or organ), a bass instrument (bass guitar or double bass), and a drummer or percussionist. In rock ensembles, usually called rock bands, there are usually guitars and keyboards (piano, electric piano, Hammond organ, synthesizer, etc.) and a rhythm section made up of a bass guitar and drum kit." .



###  http://www.semanticweb.org/musicOntology#Folk

:Folk rdf:type owl:Class ;
      
      rdfs:label "Folk" ;
      
      rdfs:subClassOf :Genre ;
      
      rdfs:comment "Folk music includes both traditional music and the genre that evolved from it during the 20th century folk revival. The term originated in the 19th century but is often applied to music that is older than that. Some types of folk music are also called world music." .



###  http://www.semanticweb.org/musicOntology#Genre

:Genre rdf:type owl:Class ;
       
       rdfs:label "Genre" ;
       
       rdfs:comment "conventional category that identifies pieces of music as belonging to a shared tradition or set of conventions" .



###  http://www.semanticweb.org/musicOntology#Hip-hop

:Hip-hop rdf:type owl:Class ;
         
         rdfs:label "Hip hop" ;
         
         rdfs:subClassOf :Genre ;
         
         rdfs:comment "Hip hop music, also called hip-hop, rap music, or hip-hop music, is a music genre consisting of a stylized rhythmic music that commonly accompanies rapping, a rhythmic and rhyming speech that is chanted. It developed as part of hip hop culture, a subculture defined by four key stylistic elements: MCing/rapping, DJing/scratching, break dancing, and graffiti writing. Other elements include sampling (or synthesis), and beatboxing. While often used to refer to rapping, \"hip hop\" more properly denotes the practice of the entire subculture. The term hip hop music is sometimes used synonymously with the term rap music, though rapping is not a required component of hip hop music; the genre may also incorporate other elements of hip hop culture, including DJing and scratching, beatboxing, and instrumental tracks." .



###  http://www.semanticweb.org/musicOntology#Idiophone

:Idiophone rdf:type owl:Class ;
           
           rdfs:label "Idiophone" ;
           
           rdfs:subClassOf :Percussion ;
           
           owl:disjointWith :Membranophone ;
           
           rdfs:comment "musical instrument, the sound source in which the body itself is a tool, or a portion thereof, is not required for pre-tensioning of sound or compression (stretched string or membrane)." .



###  http://www.semanticweb.org/musicOntology#Jazz

:Jazz rdf:type owl:Class ;
      
      rdfs:label "Jazz" ;
      
      rdfs:subClassOf :Genre ;
      
      rdfs:comment "Jazz is a genre of music that originated in African American communities during the late 19th and early 20th century. Jazz emerged in many parts of the United States of independent popular musical styles; linked by the common bonds of African American and European American musical parentage with a performance orientation. Jazz spans a range of music from ragtime to the present day—a period of over 100 years—and has proved to be very difficult to define. Jazz makes heavy use of improvisation, polyrhythms, syncopation, and the swung note, as well as aspects of European harmony, American popular music, the brass band tradition, and African musical elements such as blue notes and ragtime. A musical group that plays jazz is called a jazz band. The birth of Jazz in the multicultural society of America has lead intellectuals from around the world to refer to Jazz as \"one of America’s original art forms\"" .



###  http://www.semanticweb.org/musicOntology#KeyboardInstrument

:KeyboardInstrument rdf:type owl:Class ;
                    
                    rdfs:label "Keyboard instrument" ;
                    
                    rdfs:subClassOf :MusicalInstrument ;
                    
                    rdfs:comment "musical instruments, extract sound that made using a system of levers and controlled using keys located in a certain order and constituting a keyboard instrument." .



###  http://www.semanticweb.org/musicOntology#Latin

:Latin rdf:type owl:Class ;
       
       rdfs:label "Latin" ;
       
       rdfs:subClassOf :Genre ;
       
       rdfs:comment "Latin American music refers to music originating from Latin America namely Spanish- and Portuguese-speaking countries of the Americas and the Caribbean. Latin American music also incorporates African music from slaves who were to transported to the America by European and settles as well as music from Indigenous peoples of the Americas. The first of those encapsulates all music styles generated from Latin countries, such as salsa, merengue, tango, compas, bossa nova and bachata; as well as other styles derived from a more mainstream genre, such as Latin pop, rock, jazz and reggaeton." .



###  http://www.semanticweb.org/musicOntology#Medium

:Medium rdf:type owl:Class ;
        
        rdfs:label "Medium" ;
        
        rdfs:comment "A means or instrumentality for storing or communicating musical manifestation." .



###  http://www.semanticweb.org/musicOntology#Membranophone

:Membranophone rdf:type owl:Class ;
               
               rdfs:subClassOf :Percussion ;
               
               rdfs:comment """musical instrument in which the element produces a sound is stretched membrane.
Most membranophones drums are (but without there drums membrane made of whole piece of wood belonging to idiophone). In addition to drums, to membranophones include a special class of instruments in which the membrane alters the sound of voices.""" .



###  http://www.semanticweb.org/musicOntology#MusicalComposition

:MusicalComposition rdf:type owl:Class ;
                    
                    rdfs:label "Musical composition" ;
                    
                    rdfs:comment """Musical composition can refer to an original piece of music, the structure of a musical piece, or the process of creating a new piece of music. People who practice composition are called composers.
Although today composition is considered to consist of the manipulation of each aspect of music (harmony, melody, form, rhythm, and timbre), according to Jean-Benjamin de Laborde (1780)""" .



###  http://www.semanticweb.org/musicOntology#MusicalInstrument

:MusicalInstrument rdf:type owl:Class ;
                   
                   rdfs:label "Musical instrument" ;
                   
                   rdfs:comment "A musical instrument is an instrument created or adapted to make musical sounds. In principle, any object that produces sound can be a musical instrument—it is through purpose that the object becomes a musical instrument." .



###  http://www.semanticweb.org/musicOntology#Musician

:Musician rdf:type owl:Class ;
          
          rdfs:label "Musician" ;
          
          rdfs:comment "A musician (or instrumentalist) is a person who plays a musical instrument or is musically talented, or one who composes, conducts, or performs music." .



###  http://www.semanticweb.org/musicOntology#Nocturne

:Nocturne rdf:type owl:Class ;
          
          rdfs:label "Nocturne" ;
          
          rdfs:subClassOf :MusicalComposition ;
          
          rdfs:comment "A nocturne (from the French which meant nocturnal, from Latin nocturnus) is usually a musical composition that is inspired by, or evocative of, the night. Historically, nocturne is a very old term applied to night Offices and, since the Middle Ages, to divisions in the canonical hour of Matins." .



###  http://www.semanticweb.org/musicOntology#Occasional

:Occasional rdf:type owl:Class ;
            
            rdfs:label "Occasional" ;
            
            rdfs:subClassOf :OtherGenres ;
            
            rdfs:comment "Occasional music: Military music, marches, national anthems and related compositions" .



###  http://www.semanticweb.org/musicOntology#Octet

:Octet rdf:type owl:Class ;
       
       rdfs:label "Octet" ;
       
       rdfs:subClassOf [ rdf:type owl:Class ;
                         owl:intersectionOf ( :Collective
                                              [ rdf:type owl:Restriction ;
                                                owl:onProperty :has_member ;
                                                owl:onClass :CollectiveMember ;
                                                owl:qualifiedCardinality "8"^^xsd:nonNegativeInteger
                                              ]
                                            )
                       ] ;
       
       rdfs:comment "In music, an octet is a musical ensemble consisting of eight instruments or voices, or a musical composition written for such an ensemble." .



###  http://www.semanticweb.org/musicOntology#OtherGenres

:OtherGenres rdf:type owl:Class ;
             
             rdfs:label "Other genres" ;
             
             rdfs:subClassOf :Genre ;
             
             rdfs:comment "Music written for the score of a play, musicals, or similar: Filmi, incidental music, video game music, music hall songs and showtunes. Regional and national music with no significant commercial impact abroad, except when it is a version of an international genre, such as: traditional music, oral traditions, sea shanties, work songs, nursery rhymes, Arabesque and indigenous music" .



###  http://www.semanticweb.org/musicOntology#OtherInstruments

:OtherInstruments rdf:type owl:Class ;
                  
                  rdfs:label "Other instruments" ;
                  
                  rdfs:subClassOf :MusicalInstrument .



###  http://www.semanticweb.org/musicOntology#Percussion

:Percussion rdf:type owl:Class ;
            
            rdfs:label "Percussion" ;
            
            rdfs:subClassOf :MusicalInstrument ;
            
            rdfs:comment "group of musical instruments, the sound of which is extracted shock or vibration (swinging) [hammers, mallets, sticks, etc. n.] on the sounding body (membrane, metal, wood, etc.)." .



###  http://www.semanticweb.org/musicOntology#Performer

:Performer rdf:type owl:Class ;
           
           rdfs:label "Performer" .



###  http://www.semanticweb.org/musicOntology#Pop

:Pop rdf:type owl:Class ;
     
     rdfs:label "Pop" ;
     
     rdfs:subClassOf :Genre ;
     
     rdfs:comment "Pop music (a term that originally derives from an abbreviation of \"popular\") is a genre of popular music, which originated in its modern form in the 1950s, deriving from rock and roll. The terms \"popular music\" and \"pop music\" are often used interchangeably, although the former is a description of music which is popular (and can include any style)." .



###  http://www.semanticweb.org/musicOntology#Prelude

:Prelude rdf:type owl:Class ;
         
         rdfs:label "Prelude" ;
         
         rdfs:subClassOf :MusicalComposition ;
         
         rdfs:comment "A prelude is a short piece of music, the form of which may vary from piece to piece. The prelude may be thought of as a preface. While, during the Baroque era, for example, it may have served as an introduction to succeeding movements of a work that were usually longer and more complex, it may also have been a standalone piece of work during the Romantic era. It generally features a small number of rhythmic and melodic motifs that recur through the piece. Stylistically, the prelude is improvisatory in nature. The prelude also may refer to an overture, particularly to those seen in an opera or an oratorio." .



###  http://www.semanticweb.org/musicOntology#Quartet

:Quartet rdf:type owl:Class ;
         
         rdfs:label "Quartet" ;
         
         rdfs:subClassOf [ rdf:type owl:Class ;
                           owl:intersectionOf ( :Collective
                                                [ rdf:type owl:Restriction ;
                                                  owl:onProperty :has_member ;
                                                  owl:onClass :CollectiveMember ;
                                                  owl:qualifiedCardinality "4"^^xsd:nonNegativeInteger
                                                ]
                                              )
                         ] ;
         
         rdfs:comment "In music, a quartet or quartette (French: quatuor, German: Quartett, Italian: quartetto, Spanish: cuarteto, Polish: kwartet) is an ensemble of four singers or instrumental performers; or a musical composition for four voices or instruments." .



###  http://www.semanticweb.org/musicOntology#Quintet

:Quintet rdf:type owl:Class ;
         
         rdfs:label "Quintet" ;
         
         rdfs:subClassOf [ rdf:type owl:Class ;
                           owl:intersectionOf ( :Collective
                                                [ rdf:type owl:Restriction ;
                                                  owl:onProperty :has_member ;
                                                  owl:onClass :CollectiveMember ;
                                                  owl:qualifiedCardinality "5"^^xsd:nonNegativeInteger
                                                ]
                                              )
                         ] ;
         
         rdfs:comment "A quintet is a group containing five members. It is commonly associated with musical groups, such as a string quintet, or a group of five singers, but can be applied to any situation where five similar or related objects are considered a single unit. In classical instrumental music, any additional instrument (such as a piano, clarinet, oboe, etc.) joined to the usual string quartet (two violins, a viola, and a cello), gives the resulting ensemble its name, such as \"piano quintet\", \"clarinet quintet\", etc. A piece of music written for such a group is similarly named." .



###  http://www.semanticweb.org/musicOntology#R&B-and-soul

<http://www.semanticweb.org/musicOntology#R&B-and-soul> rdf:type owl:Class ;
                                                        
                                                        rdfs:label "R&B and soul" ;
                                                        
                                                        rdfs:subClassOf :Genre ;
                                                        
                                                        rdfs:comment "Rhythm and blues, often abbreviated as R&B or RnB, is a genre of popular African-American music that originated in the 1940s. The term was originally used by record companies to describe recordings marketed predominantly to urban African Americans, at a time when \"urbane, rocking, jazz based music with a heavy, insistent beat\" was becoming more popular. In the commercial rhythm and blues music typical of the 1950s through the 1970s, the bands usually consisted of piano, one or two guitars, bass, drums, saxophone, and sometimes background vocalists. R&B lyrical themes often encapsulate the African-American experience of pain and the quest for freedom and joy. Lyrics focus heavily on the themes of triumphs and failures in terms of relationships, freedom, economics, aspirations, and sex." .



###  http://www.semanticweb.org/musicOntology#Religious

:Religious rdf:type owl:Class ;
           
           rdfs:label "Religious" ;
           
           rdfs:subClassOf :Genre .



###  http://www.semanticweb.org/musicOntology#Rock

:Rock rdf:type owl:Class ;
      
      rdfs:label "Rock" ;
      
      rdfs:subClassOf :Genre ;
      
      rdfs:comment "Rock music is a genre of popular music that originated as \"rock and roll\" in the United States in the 1950s, and developed into a range of different styles in the 1960s and later, particularly in the United Kingdom and the United States. It has its roots in 1940s' and 1950s' rock and roll, itself heavily influenced by rhythm and blues and country music. Rock music also drew strongly on a number of other genres such as blues and folk, and incorporated influences from jazz, classical and other musical sources." .



###  http://www.semanticweb.org/musicOntology#Septet

:Septet rdf:type owl:Class ;
        
        rdfs:label "Septet" ;
        
        rdfs:subClassOf [ rdf:type owl:Class ;
                          owl:intersectionOf ( :Collective
                                               [ rdf:type owl:Restriction ;
                                                 owl:onProperty :has_member ;
                                                 owl:onClass :CollectiveMember ;
                                                 owl:qualifiedCardinality "7"^^xsd:nonNegativeInteger
                                               ]
                                             )
                        ] ;
        
        rdfs:comment "A septet is a formation containing exactly seven members. It is commonly associated with musical groups, but can be applied to any situation where seven similar or related objects are considered a single unit, such as a seven-line stanza of poetry." .



###  http://www.semanticweb.org/musicOntology#Sextet

:Sextet rdf:type owl:Class ;
        
        rdfs:label "Sextet" ;
        
        rdfs:subClassOf [ rdf:type owl:Class ;
                          owl:intersectionOf ( :Collective
                                               [ rdf:type owl:Restriction ;
                                                 owl:onProperty :has_member ;
                                                 owl:onClass :CollectiveMember ;
                                                 owl:qualifiedCardinality "6"^^xsd:nonNegativeInteger
                                               ]
                                             )
                        ] ;
        
        rdfs:comment "A sextet (or hexad) is a formation containing exactly six members. It is commonly associated with vocal or musical instrument groups, but can be applied to any situation where six similar or related objects are considered a single unit." .



###  http://www.semanticweb.org/musicOntology#SoloPerformer

:SoloPerformer rdf:type owl:Class ;
               
               rdfs:label "Solo performer" ;
               
               rdfs:subClassOf [ rdf:type owl:Class ;
                                 owl:intersectionOf ( :Performer
                                                      [ rdf:type owl:Restriction ;
                                                        owl:onProperty :musician ;
                                                        owl:onClass :Musician ;
                                                        owl:qualifiedCardinality "1"^^xsd:nonNegativeInteger
                                                      ]
                                                    )
                               ] .



###  http://www.semanticweb.org/musicOntology#Sonata

:Sonata rdf:type owl:Class ;
        
        rdfs:label "Sonata" ;
        
        rdfs:subClassOf :MusicalComposition ;
        
        rdfs:comment "Sonata, in music, literally means a piece played as opposed to a cantata (Latin and Italian cantare, \"to sing\"), a piece sung. The term, being vague, evolved through the history of music, designating a variety of forms until the Classical era, when it took on increasing importance, and by the early 19th century came to represent a principle of composing large scale works. It was applied to most instrumental genres and regarded—alongside the fugue—as one of two fundamental methods of organizing, interpreting and analyzing concert music. Though the musical style of sonatas has changed since the Classical era, most 20th- and 21st-century sonatas still maintain the same structure." .



###  http://www.semanticweb.org/musicOntology#Song

:Song rdf:type owl:Class ;
      
      rdfs:label "Song" ;
      
      rdfs:subClassOf :MusicalComposition ;
      
      rdfs:comment "In music, a song is a composition for voice performed by singing or alongside musical instruments. A choral or vocal song may be accompanied by musical instruments, or it may be unaccompanied, as in the case of a cappella songs. The lyrics (words) of songs are typically of a poetic, rhyming nature, though they may be religious verses or free prose." .



###  http://www.semanticweb.org/musicOntology#South-and-southeastAsian

:South-and-southeastAsian rdf:type owl:Class ;
                          
                          rdfs:label "South and southeast Asian" ;
                          
                          rdfs:subClassOf :Asian ;
                          
                          rdfs:comment "Southeast Asian music include the musical traditions of this subregion of Asia. This subregion consists of eleven countries, namely, Brunei, Cambodia, East Timor, Indonesia, Laos, Malaysia, Myanmar, Philippines, Singapore, Thailand, Vietnam, and Northeast India." .



###  http://www.semanticweb.org/musicOntology#Symphony

:Symphony rdf:type owl:Class ;
          
          rdfs:label "Symphony" ;
          
          rdfs:subClassOf :MusicalComposition ;
          
          rdfs:comment "A symphony is an extended musical composition in Western classical music, most often written for orchestra. Although the term has had many meanings from its origins in the ancient Greek era, by the late 18th century the word had taken on the meaning common today: a work usually consisting of multiple distinct sections or movements, often four, with the first movement in sonata form." .



###  http://www.semanticweb.org/musicOntology#Trio

:Trio rdf:type owl:Class ;
      
      rdfs:label "Trio" ;
      
      rdfs:subClassOf [ rdf:type owl:Class ;
                        owl:intersectionOf ( :Collective
                                             [ rdf:type owl:Restriction ;
                                               owl:onProperty :has_member ;
                                               owl:onClass :CollectiveMember ;
                                               owl:qualifiedCardinality "3"^^xsd:nonNegativeInteger
                                             ]
                                           )
                      ] ;
      
      rdfs:comment "In music, a trio (an Italian word) is a method of instrumentation or vocalization by three different sounds or voices to make a melodious music or song." .





#################################################################
#
#    Individuals
#
#################################################################


###  http://www.semanticweb.org/musicOntology#10YearsToday

<http://www.semanticweb.org/musicOntology#10YearsToday> rdf:type :Song ,
                                                                 owl:NamedIndividual ;
                                                        
                                                        rdfs:label "10 Years Today" ;
                                                        
                                                        :performer :BulletForMyValentine ;
                                                        
                                                        :composer :BulletForMyValentine ;
                                                        
                                                        :from_album :ThePoison .



###  http://www.semanticweb.org/musicOntology#4Words

<http://www.semanticweb.org/musicOntology#4Words> rdf:type :Song ,
                                                           owl:NamedIndividual ;
                                                  
                                                  rdfs:label "4 Words" ;
                                                  
                                                  :performer :BulletForMyValentine ;
                                                  
                                                  :composer :BulletForMyValentine ;
                                                  
                                                  :from_album :ThePoison .



###  http://www.semanticweb.org/musicOntology#APlaceForMyHead

:APlaceForMyHead rdf:type :Song ,
                          owl:NamedIndividual ;
                 
                 rdfs:label "A Place For My Head" ;
                 
                 :performer :LinkinPark ;
                 
                 :composer :LinkinPark .



###  http://www.semanticweb.org/musicOntology#AdultContemporary

:AdultContemporary rdf:type :Pop ,
                            owl:NamedIndividual ;
                   
                   rdfs:label "Adult contemporary" ;
                   
                   rdfs:comment "Adult contemporary music (AC) is a style of music, ranging from 1960s vocal and 1970s soft rock music to predominantly ballad-heavy music of the present day, with varying degrees of easy listening, soul, rhythm and blues, and rock influence. Adult contemporary is rather a continuation of the easy listening and soft rock style that became popular in the 1960s and 1970s with some adjustments that reflect the evolution of pop/rock music." .



###  http://www.semanticweb.org/musicOntology#Afrobeat

:Afrobeat rdf:type :African ,
                   owl:NamedIndividual ;
          
          rdfs:label "Afrobeat" ;
          
          rdfs:comment "Afrobeat is a combination of traditional Nigerian and Ghanaian music, jazz, highlife, funk, and chanted vocals,[1] fused with percussion and vocal styles, popularised in Africa in the 1970s." .



###  http://www.semanticweb.org/musicOntology#AllTheseThingsIHate

:AllTheseThingsIHate rdf:type :Song ,
                              owl:NamedIndividual ;
                     
                     rdfs:label "All These Things I Hate" ;
                     
                     :composer :BulletForMyValentine ;
                     
                     :performer :BulletForMyValentine ;
                     
                     :from_album :ThePoison .



###  http://www.semanticweb.org/musicOntology#AllWeAre

:AllWeAre rdf:type :Song ,
                   owl:NamedIndividual ;
          
          rdfs:label "All We Are" .



###  http://www.semanticweb.org/musicOntology#AlternativeRock

:AlternativeRock rdf:type :Rock ,
                          owl:NamedIndividual ;
                 
                 rdfs:label "Alternative rock" ;
                 
                 rdfs:comment "Alternative rock (also called alternative music, alt-rock or simply alternative) is a genre of rock music that emerged from the independent music underground of the 1980s and became widely popular by the 1990s. The \"alternative\" definition refers to the genre's distinction from mainstream rock music, expressed primarily in a distorted guitar sound, subversive and/or transgressive lyrics and generally a nonchalant, defiant attitude. The term's original meaning was broader, referring to a generation of musicians unified by their collective debt to either the musical style, or simply the independent, D.I.Y. ethos of punk rock, which in the late 1970s laid the groundwork for alternative music. At times, \"alternative\" has been used as a catch-all description for music from underground rock artists that receives mainstream recognition, or for any music, whether rock or not, that is seen to be descended from punk rock (including some examples of punk itself, as well as new wave, and post-punk)." .



###  http://www.semanticweb.org/musicOntology#AndreaBocelli

:AndreaBocelli rdf:type :Musician ,
                        owl:NamedIndividual ;
               
               rdfs:label "Andrea Bocelli" ;
               
               :name "Andrea Bocelli" .



###  http://www.semanticweb.org/musicOntology#Anison

:Anison rdf:type :EastAsian ,
                 owl:NamedIndividual ;
        
        rdfs:label "Anison" .



###  http://www.semanticweb.org/musicOntology#AudioFile

:AudioFile rdf:type :Medium ,
                    owl:NamedIndividual ;
           
           rdfs:label "Audio file" ;
           
           rdfs:comment "An audio file, which may be available on a local file system or through http, ftp, etc." .



###  http://www.semanticweb.org/musicOntology#BFMV-MatthewTuck

:BFMV-MatthewTuck rdf:type :CollectiveMember ,
                           owl:NamedIndividual ;
                  
                  :collectiveRole :InstrumentPlayer ;
                  
                  :musician :MatthewTuck ;
                  
                  :collectiveRole :Vocal .



###  http://www.semanticweb.org/musicOntology#BFMV-MichaelPaget

:BFMV-MichaelPaget rdf:type :CollectiveMember ,
                            owl:NamedIndividual ;
                   
                   :collectiveRole :InstrumentPlayer ;
                   
                   :musician :MichaelPaget ;
                   
                   :collectiveRole :Vocal .



###  http://www.semanticweb.org/musicOntology#BFMV-MichaelThomas

:BFMV-MichaelThomas rdf:type :CollectiveMember ,
                             owl:NamedIndividual ;
                    
                    :collectiveRole :InstrumentPlayer ;
                    
                    :musician :MichaelThomas .



###  http://www.semanticweb.org/musicOntology#BackgroundMusic

:BackgroundMusic rdf:type :Easy-listening ,
                          owl:NamedIndividual ;
                 
                 rdfs:label "Background music" ;
                 
                 rdfs:comment "Background music refers to various styles of music or soundscapes primarily intended to be passively listened to. It is not meant to be the main focus of an audience, but rather to supplement that which is meant to be focused upon. Music that is played at a low volume and is not the main focus of an audience is also referred to as background music. Traditional examples of background music include music played at various social gatherings and music played in certain retail venues. It is also common to employ background music in various electronic media including film, television, and Internet videos such as video blogs." .



###  http://www.semanticweb.org/musicOntology#Baila

:Baila rdf:type :South-and-southeastAsian ,
                owl:NamedIndividual ;
       
       rdfs:label "Baila" ;
       
       rdfs:comment "Bayila (also known as baila) is a form of music, popular in Sri Lanka and parts of India. The genre originated centuries ago among the 'Sri Lankan Kaffirs' or Afro-Sinhalese communities (mixed communities of Portuguese, African and native Sinhalese people). It primarily utilises European instruments and rhythms found in Spain/Portugal, Sri Lanka, Africa and South India. Bayila songs are played during parties and weddings in Mangalore and Goa, accompanied by dancing." .



###  http://www.semanticweb.org/musicOntology#Balalaika

:Balalaika rdf:type :Chordophone ,
                    owl:NamedIndividual ;
           
           rdfs:label "Balalaika" ;
           
           rdfs:comment "The balalaika is a Russian stringed musical instrument with a characteristic triangular body and three strings." .



###  http://www.semanticweb.org/musicOntology#BassGuitar

:BassGuitar rdf:type :Chordophone ,
                     owl:NamedIndividual ;
            
            rdfs:label "Bass guitar" ;
            
            rdfs:comment "The bass guitar (also called electric bass, or simply bass; /ˈbeɪs/) is a stringed instrument played primarily with the fingers or thumb, by plucking, slapping, popping, (rarely) strumming, tapping, thumping, or picking with a plectrum, often known as a pick." .



###  http://www.semanticweb.org/musicOntology#Bebop

:Bebop rdf:type :Jazz ,
                owl:NamedIndividual ;
       
       rdfs:label "Bebop" ;
       
       rdfs:comment "Bebop or bop is a style of jazz characterized by a fast tempo, instrumental virtuosity, and improvisation based on the combination of harmonic structure and sometimes references to the melody. It was developed in the early and mid-1940s. This style of jazz ultimately became synonymous with modern jazz, as either category reached a certain final maturity in the 1960s." .



###  http://www.semanticweb.org/musicOntology#BetterOffAlone

:BetterOffAlone rdf:type :Song ,
                         owl:NamedIndividual ;
                
                rdfs:label "Better Off Alone" ;
                
                :performer :BulletForMyValentine ;
                
                :composer :BulletForMyValentine .



###  http://www.semanticweb.org/musicOntology#BetterOffAlone(EP)

<http://www.semanticweb.org/musicOntology#BetterOffAlone(EP)> rdf:type :Album ,
                                                                       owl:NamedIndividual ;
                                                              
                                                              rdfs:label "Better Off Alone (EP)" ;
                                                              
                                                              rdfs:comment "Better Off Alone is the first ever EP released by Welsh band \"Jeff Killed John\", known today as Bullet for My Valentine. In its initial phase, the boys wrote few songs of their own and played a lot of covers, most notably Metallica and Nirvana songs. When they began to start writing their own songs, Better Off Alone was released in 1999 with their first four songs." ;
                                                              
                                                              :has_song :BetterOffAlone ,
                                                                        :BottomOfTheLine ;
                                                              
                                                              :performer :BulletForMyValentine ;
                                                              
                                                              :recorded_on :CD ,
                                                                           :DVD-Audio ;
                                                              
                                                              :has_song :DontWalkAway ,
                                                                        :WrongOfMe .



###  http://www.semanticweb.org/musicOntology#BillieJean

:BillieJean rdf:type :Song ,
                     owl:NamedIndividual ;
            
            rdfs:label "Billie Jean" ;
            
            :recorded_on :CD ,
                         :DAT ,
                         :DCC ;
            
            :composer :MichaelJackson ;
            
            :performer :Solo-MichaelJackson .



###  http://www.semanticweb.org/musicOntology#Bolero

:Bolero rdf:type :Latin ,
                 owl:NamedIndividual ;
        
        rdfs:label "Bolero" ;
        
        rdfs:comment "Bolero is a genre of slow-tempo Latin music and its associated dance. There are Spanish and Cuban forms which are both significant and which have separate origins." .



###  http://www.semanticweb.org/musicOntology#Bongo

:Bongo rdf:type :Membranophone ,
                owl:NamedIndividual ;
       
       rdfs:label "Bongo drum" ;
       
       rdfs:comment "Bongos (Spanish: bongó) are an Afro-Cuban percussion instrument consisting of a pair of small open bottomed drums of different sizes. In Spanish the larger drum is called the hembra (female) and the smaller the macho (male). They are membranophones, or instruments that create sound by a vibration of a stretched membrane." .



###  http://www.semanticweb.org/musicOntology#BottomOfTheLine

:BottomOfTheLine rdf:type :Song ,
                          owl:NamedIndividual ;
                 
                 rdfs:label "Bottom of the Line" ;
                 
                 :composer :BulletForMyValentine ;
                 
                 :performer :BulletForMyValentine .



###  http://www.semanticweb.org/musicOntology#BradDelson

:BradDelson rdf:type :Musician ,
                     owl:NamedIndividual ;
            
            rdfs:label "Bradford Delson" ;
            
            :name "Bradford Phillip \"Brad\" Delson" ;
            
            rdfs:comment "Bradford Phillip \"Brad\" Delson (born December 1, 1977) is an American musician, best known as the guitarist and one of the founding members of the Grammy Award winning rock band Linkin Park. He is also the A&R Representative for Machine Shop Recordings." ;
            
            :plays_on :BassGuitar ,
                      :Drums ,
                      :ElectricGuitar ;
            
            :primaryMusicalInstrument :ElectricGuitar .



###  http://www.semanticweb.org/musicOntology#BulletForMyValentine

:BulletForMyValentine rdf:type :Trio ,
                               owl:NamedIndividual ;
                      
                      rdfs:label "Bullet for My Valentine" ;
                      
                      rdfs:comment "Bullet for My Valentine are a Welsh heavy metal band from Bridgend, formed in 1998. The band is composed of Matthew Tuck (lead vocals, rhythm guitar), Michael Paget (lead guitar, backing vocals), and Michael Thomas (drums). Former members include Nick Crandle and Jason James; both were on bass. They were formed under the name Jeff Killed John and started their music career by covering songs by Metallica and Nirvana. Jeff Killed John recorded six songs which were not released; two of these tracks were reworked later in their career as Bullet for My Valentine. Financial difficulties dictated the name change, which was followed by a change in music direction. In 2002, the band secured a five-album deal with Sony BMG. The band has stated that their music is influenced by classic metal acts such as Metallica, Iron Maiden, and Slayer. The band is part of the Cardiff music scene." ;
                      
                      :has_member :BFMV-MatthewTuck ,
                                  :BFMV-MichaelPaget ,
                                  :BFMV-MichaelThomas ;
                      
                      :has_album <http://www.semanticweb.org/musicOntology#BetterOffAlone(EP)> ;
                      
                      :has_genre :HeavyMetal ;
                      
                      :has_album :ThePoison .



###  http://www.semanticweb.org/musicOntology#ByMyself

:ByMyself rdf:type :Song ,
                   owl:NamedIndividual ;
          
          rdfs:label "By Myself" ;
          
          :performer :LinkinPark ;
          
          :composer :LinkinPark .



###  http://www.semanticweb.org/musicOntology#CD

:CD rdf:type :Medium ,
             owl:NamedIndividual ;
    
    rdfs:label "Compact Disc" ;
    
    rdfs:comment "Compact Disc used as medium to record a musical manifestation." .



###  http://www.semanticweb.org/musicOntology#Castanets

:Castanets rdf:type :Idiophone ,
                    owl:NamedIndividual ;
           
           rdfs:label "Castanets" ;
           
           rdfs:comment "Castanets are a percussion instrument (idiophone), used in Kalo, Moorish, Ottoman, ancient Roman, Italian, Spanish, Sephardic, Swiss, and Portuguese music. The instrument consists of a pair of concave shells joined on one edge by a string. They are held in the hand and used to produce clicks for rhythmic accents or a ripping or rattling sound consisting of a rapid series of clicks. They are traditionally made of hardwood (chestnut; Spanish: castaño), although fibreglass is becoming increasingly popular." .



###  http://www.semanticweb.org/musicOntology#Cha-cha-cha

:Cha-cha-cha rdf:type :BallroomDance ,
                      owl:NamedIndividual ;
             
             rdfs:label "Cha cha cha" ;
             
             rdfs:comment "Cha-cha-chá is a genre of Cuban music. It has been a popular dance music which developed from the danzón in the early 1950s, and became widely popular throughout Cuba, Mexico and New York City." .



###  http://www.semanticweb.org/musicOntology#Chanson

:Chanson rdf:type :Pop ,
                  owl:NamedIndividual ;
         
         rdfs:label "Chanson" ;
         
         rdfs:comment "A chanson is in general any lyric-driven French song, usually polyphonic and secular. A singer specializing in chansons is known as a \"chanteur\" (male) or \"chanteuse\" (female); a collection of chansons, especially from the late Middle Ages and Renaissance, is also known as a chansonnier." .



###  http://www.semanticweb.org/musicOntology#ChesterBennington

:ChesterBennington rdf:type :Musician ,
                            owl:NamedIndividual ;
                   
                   rdfs:label "Chester Bennington" ;
                   
                   :name "Chester Charles Bennington" ;
                   
                   rdfs:comment "Chester Charles Bennington is an American musician, singer, songwriter, and actor. He is best known as the lead vocalist of rock bands Linkin Park and Dead by Sunrise. He was originally the lead vocalist for Sean Dowdell And His Friends? and Grey Daze. He is also the current lead vocalist for Stone Temple Pilots and rock cover band Bucket of Weenies." .



###  http://www.semanticweb.org/musicOntology#Chimurenga

:Chimurenga rdf:type :African ,
                     owl:NamedIndividual ;
            
            rdfs:label "Chimurenga" ;
            
            rdfs:comment "Chimurenga music is a Zimbabwean popular music genre coined and popularized by Thomas Mapfumo" .



###  http://www.semanticweb.org/musicOntology#Clarinet

:Clarinet rdf:type :Aerophone ,
                   owl:NamedIndividual ;
          
          rdfs:label "Clarinet" ;
          
          rdfs:comment "The clarinet is a family of woodwind instruments that have a single-reed mouthpiece, a straight cylindrical tube with an approximately cylindrical bore, and a flaring bell. A person who plays any type of clarinet is called a clarinetist or clarinettist." .



###  http://www.semanticweb.org/musicOntology#Clavinet

:Clavinet rdf:type :KeyboardInstrument ,
                   owl:NamedIndividual ;
          
          rdfs:label "Clavinet" ;
          
          rdfs:comment "The Clavinet is an electrically amplified clavichord that was manufactured by the Hohner company of Trossingen, West Germany from 1964 to the early 1980s. Hohner produced seven models over the years, designated I, II, L, C, D6, E7 and Duo. Its distinctive bright staccato sound has appeared particularly in funk, disco, rock, and reggae songs." .



###  http://www.semanticweb.org/musicOntology#ConTePartiro

:ConTePartiro rdf:type :Song ,
                       owl:NamedIndividual ;
              
              rdfs:label "Con te Partiro" ;
              
              :composer :AndreaBocelli ;
              
              :recorded_on :MagneticTape ;
              
              :performer :Solo-AndreaBocelli ;
              
              :recorded_on :Vinyl .



###  http://www.semanticweb.org/musicOntology#ContemporaryR&B

<http://www.semanticweb.org/musicOntology#ContemporaryR&B> rdf:type :Blues ,
                                                                    owl:NamedIndividual ;
                                                           
                                                           rdfs:label "Contemporary R&B" ;
                                                           
                                                           rdfs:comment "Contemporary R&B, also known as simply R&B, is a music genre that combines elements of rhythm and blues, soul, funk, pop, hip hop and dance." .



###  http://www.semanticweb.org/musicOntology#Crawling

:Crawling rdf:type :Song ,
                   owl:NamedIndividual ;
          
          rdfs:label "Crawling" ;
          
          :composer :LinkinPark ;
          
          :performer :LinkinPark .



###  http://www.semanticweb.org/musicOntology#Crunkcore

:Crunkcore rdf:type :Hip-hop ,
                    owl:NamedIndividual ;
           
           rdfs:label "Crunkcore" ;
           
           rdfs:comment "Crunkcore (also called crunk punk, screamo crunk, crunk rock, and scrunk) is a musical genre that combines crunk hip hop with the vocal style of screamo" .



###  http://www.semanticweb.org/musicOntology#Crystallophone

:Crystallophone rdf:type :OtherInstruments ,
                         owl:NamedIndividual ;
                
                rdfs:label "Crystallophone" ;
                
                rdfs:comment "A crystallophone is a musical instrument that produces sound from glass." .



###  http://www.semanticweb.org/musicOntology#CureForTheItch

:CureForTheItch rdf:type :Song ,
                         owl:NamedIndividual ;
                
                rdfs:label "Cure For The Itch" ;
                
                :performer :LinkinPark ;
                
                :composer :LinkinPark .



###  http://www.semanticweb.org/musicOntology#DAT

:DAT rdf:type :Medium ,
              owl:NamedIndividual ;
     
     rdfs:label "Digital Audio Tape" ;
     
     rdfs:comment "Digital Audio Tape used as medium to record a musical manifestation" .



###  http://www.semanticweb.org/musicOntology#DCC

:DCC rdf:type :Medium ,
              owl:NamedIndividual ;
     
     rdfs:label "Digital Compact Cassette" ;
     
     rdfs:comment "Digital Compact Cassette used as medium to record a musical manifestation." .



###  http://www.semanticweb.org/musicOntology#DVD-Audio

:DVD-Audio rdf:type :Medium ,
                    owl:NamedIndividual ;
           
           rdfs:label "DVD-Audio" ;
           
           rdfs:comment "DVD-Audio used as medium to record a musical manifestation." .



###  http://www.semanticweb.org/musicOntology#Dance-pop

:Dance-pop rdf:type :Pop ,
                    owl:NamedIndividual ;
           
           rdfs:label "Dance-pop" ;
           
           rdfs:comment "Dance-pop is dance-oriented pop music that originated in the early 1980s. Developing from post-disco, synthpop, and electropop, it is generally up-tempo music intended for clubs with the intention of being danceable but also suitable for contemporary hit radio. Dance-pop music is generally characterised by strong beats with easy, uncomplicated song structures which are generally more similar to pop music than the more free-form dance genre, with an emphasis on melody as well as catchy tunes. The genre, on the whole, tends to be producer-driven, despite some notable exceptions." .



###  http://www.semanticweb.org/musicOntology#DaveFarrell

:DaveFarrell rdf:type :Musician ,
                      owl:NamedIndividual ;
             
             rdfs:label "Dave Farrell" ;
             
             rdfs:comment "David Michael \"Phoenix\" Farrell (born February 8, 1977 in Plymouth, Massachusetts) is the bass guitarist of the band Linkin Park. He is an American musician, and multi-instrumentalist." ;
             
             :name "David Michael \"Phoenix\" Farrell" ;
             
             :primaryMusicalInstrument :BassGuitar ;
             
             :plays_on :BassGuitar .



###  http://www.semanticweb.org/musicOntology#Disco

:Disco rdf:type <http://www.semanticweb.org/musicOntology#R&B-and-soul> ,
                owl:NamedIndividual ;
       
       rdfs:label "Disco" ;
       
       rdfs:comment "Disco is a genre of music containing elements of funk, soul, pop, salsa and psychedelic that was most popular in the 1970s, though it has since enjoyed brief resurgences. The term is derived from discotheque (French for \"library of phonograph records\", but subsequently used as proper name for nightclubs in Paris). Its initial audiences were club-goers from the African American,  Italian American, Latino, and psychedelic communities in New York City and Philadelphia during the late 1960s and early 1970s. Disco also was a reaction against both the domination of rock music and the stigmatization of dance music by the counterculture during this period. Women embraced disco as well, and the music eventually expanded to several other popular groups of the time." .



###  http://www.semanticweb.org/musicOntology#Dixieland

:Dixieland rdf:type :Jazz ,
                    owl:NamedIndividual ;
           
           rdfs:label "Dixieland" ;
           
           rdfs:comment "Dixieland music or New Orleans Jazz, sometimes referred to as Hot jazz or Early Jazz, is a style of jazz music which developed in New Orleans at the start of the 20th century, and was spread to Chicago and New York City by New Orleans bands in the 1910s. Well-known jazz standard songs from the Dixieland era, such as \"Basin Street Blues\" and \"When the Saints Go Marching In\", are known even to non-jazz fans. With its beginnings in Dixieland and Riverboat jazz, and progression to Chicago-style jazz or hot jazz as developed by Louis Armstrong and others. Chicago-style jazz or hot jazz was also a transition and combination of 2-beat to 4-beat, introducing Swing in its earliest form. \"Chicago style\" musicians used the string bass instead of the tuba and the guitar instead of the banjo to play a faster-paced, swinging style that emphasized solos. Hot jazz or Chicago-style jazz was also the current original music that began the Lindy Hop dance craze as it developed in Harlem." .



###  http://www.semanticweb.org/musicOntology#DontStopTilYouGetEnough

:DontStopTilYouGetEnough rdf:type :Song ,
                                  owl:NamedIndividual ;
                         
                         rdfs:label "Dont Stop Til You Get Enough" ;
                         
                         :recorded_on :CD ,
                                      :MagneticTape ;
                         
                         :composer :MichaelJackson ;
                         
                         :performer :Solo-MichaelJackson .



###  http://www.semanticweb.org/musicOntology#DontWalkAway

:DontWalkAway rdf:type :Song ,
                       owl:NamedIndividual ;
              
              rdfs:label "Dont Walk Away" ;
              
              :composer :BulletForMyValentine ;
              
              :performer :BulletForMyValentine .



###  http://www.semanticweb.org/musicOntology#Drums

:Drums rdf:type :Membranophone ,
                owl:NamedIndividual ;
       
       rdfs:label "Drum kit" ;
       
       rdfs:comment """A drum kit, drum set or trap set is a collection of drums and other percussion instruments set up to be played/struck by a single player.
The traditional drum kit consists of a mix of drums (classified as classically as membranophones, Hornbostel-Sachs high-level classification 2) and idiophones (Hornbostel-Sachs high-level classification 1, most significantly cymbals but also including the woodblock and cowbell for example).[3] More recently kits have also included electronic instruments (Hornbostel-Sachs classification 53), with both hybrid and entirely electronic kits now in common use.""" .



###  http://www.semanticweb.org/musicOntology#ElectricGuitar

:ElectricGuitar rdf:type :Chordophone ,
                         owl:NamedIndividual ;
                
                rdfs:label "Electric guitar" ;
                
                rdfs:comment "An electric guitar is a guitar that uses a pickup to convert the vibration of its strings into electrical impulses. The most common guitar pickup uses the principle of direct electromagnetic induction. The signal generated by an electric guitar is too weak to drive a loudspeaker, so it is amplified before sending it to a loudspeaker. Since the output of an electric guitar is an electric signal, the signal may easily be altered using electronic circuits to add \"color\" to the sound. Often the signal is modified using effects such as reverb and distortion." .



###  http://www.semanticweb.org/musicOntology#Electroacoustic

:Electroacoustic rdf:type :Avant-garde ,
                          owl:NamedIndividual ;
                 
                 rdfs:label "Electroacoustic" ;
                 
                 rdfs:comment "Electroacoustic music originated in Western art music during the modern era following the incorporation of electric sound production into compositional practice." .



###  http://www.semanticweb.org/musicOntology#ElevatorMusic

:ElevatorMusic rdf:type :Easy-listening ,
                        owl:NamedIndividual ;
               
               rdfs:label "Elevator music" ;
               
               rdfs:comment "Elevator music (also known as Muzak, piped music, weather music, or lift music) refers to a type of popular music, often instrumental, that is commonly played through speakers at shopping malls, grocery stores, department stores, telephone systems (while the caller is on hold), cruise ships, airliners (during take-off and flight), hotels, airports, business offices, hospitals, and elevators. As well as television program menu, weather forecast and test card. The term is also frequently applied as a generic term for any form of easy listening, smooth jazz, or middle of the road music, or to the type of recordings commonly heard on \"beautiful music\" radio stations." .



###  http://www.semanticweb.org/musicOntology#Eminem

:Eminem rdf:type :Musician ,
                 owl:NamedIndividual ;
        
        rdfs:label "Eminem" ;
        
        :name "Marshall Bruce Mathers III" ;
        
        rdfs:comment "Marshall Bruce Mathers III (born October 17, 1972), best known by his stage name Eminem, is an American rapper, record producer, songwriter, and actor. In addition to his solo career, Eminem is a member of the group D12, as well as one half of the hip hop duo Bad Meets Evil, alongside Royce da 5'9\". Eminem is the best-selling artist of the 2000s in the United States. Rolling Stone magazine ranked him 83rd on its list of The 100 Greatest Artists of All Time. The same magazine declared him The King of Hip Hop. Including his work with D12 and Bad Meets Evil, Eminem has achieved ten number-one albums on the Billboard 200. Eminem has sold more than 155 million albums and singles, making him one of the world's best-selling artists of all time. As of June 2014, he is the second best-selling male artist of the Nielsen SoundScan era, the sixth-best overall selling artist in the United States, and the best-selling hip-hop artist, having sold 45,160,000 albums and 31 million digital singles." .



###  http://www.semanticweb.org/musicOntology#Enka

:Enka rdf:type :EastAsian ,
               owl:NamedIndividual ;
      
      rdfs:label "Enka" ;
      
      rdfs:comment "is a popular Japanese music genre considered to resemble traditional Japanese music stylistically." .



###  http://www.semanticweb.org/musicOntology#EveryGirlLikeMe

:EveryGirlLikeMe rdf:type :Song ,
                          owl:NamedIndividual ;
                 
                 rdfs:label "Every Girl Like Me" .



###  http://www.semanticweb.org/musicOntology#ExperimentalMusic

:ExperimentalMusic rdf:type :Avant-garde ,
                            owl:NamedIndividual ;
                   
                   rdfs:label "Experimental music" ;
                   
                   rdfs:comment "Experimental music is a compositional tradition that arose in the mid-20th century, particularly in North America, of music composed in such a way that its outcome is unforeseeable." .



###  http://www.semanticweb.org/musicOntology#Flute

:Flute rdf:type :Aerophone ,
                owl:NamedIndividual ;
       
       rdfs:label "Flute" ;
       
       rdfs:comment "The flute is a family of musical instrument of the woodwind group. Unlike woodwind instruments with reeds, a flute is an aerophone or reedless wind instrument that produces its sound from the flow of air across an opening. According to the instrument classification of Hornbostel–Sachs, flutes are categorized as edge-blown aerophones." .



###  http://www.semanticweb.org/musicOntology#Forgotten

:Forgotten rdf:type :Song ,
                    owl:NamedIndividual ;
           
           rdfs:label "Forgotten" ;
           
           :composer :LinkinPark ;
           
           :performer :LinkinPark .



###  http://www.semanticweb.org/musicOntology#Freakfolk

:Freakfolk rdf:type :Folk ,
                    owl:NamedIndividual ;
           
           rdfs:label "Freak folk" ;
           
           rdfs:comment "Freak folk is a genre of folk music which uses mainly acoustic instrumentation, but introduces elements of avant-garde music, baroque pop, and psychedelic folk, often featuring uncommon sounds, lyrical themes, and vocal styles." .



###  http://www.semanticweb.org/musicOntology#Frevo

:Frevo rdf:type :Brazilian ,
                owl:NamedIndividual ;
       
       rdfs:label "Frevo" ;
       
       rdfs:comment "Frevo is a wide range of musical styles originating from Recife, Pernambuco, Brazil, all of which are traditionally associated with Brazilian Carnival. The word frevo is said to come from frever, a misspeaking of the Portuguese word ferver (to boil). It is said that the sound of the frevo will make listeners and dancers feel as if they are boiling on the ground. The word frevo is used for both the frevo music and the frevo dance." .



###  http://www.semanticweb.org/musicOntology#Funk

:Funk rdf:type <http://www.semanticweb.org/musicOntology#R&B-and-soul> ,
               owl:NamedIndividual ;
      
      rdfs:label "Funk" ;
      
      rdfs:comment "Funk is a music genre that originated in the mid to late 1960s when African-American musicians created a rhythmic, danceable new form of music through a mixture of soul music, jazz, and R&B. Funk de-emphasizes melody and harmony and brings a strong rhythmic groove of electric bass and drums to the foreground. Funk songs are often based on an extended vamp on a single chord, distinguishing them from R&B and soul songs, which are built on chord progressions. Funk uses the same extended chords found in bebop jazz, such as minor chords with added sevenths and elevenths, or dominant seventh chords with altered ninths." .



###  http://www.semanticweb.org/musicOntology#GregorianChant

:GregorianChant rdf:type :Religious ,
                         owl:NamedIndividual ;
                
                rdfs:label "Gregorian chant" ;
                
                rdfs:comment "Gregorian chant is the central tradition of Western plainchant, a form of monophonic, unaccompanied sacred song of the western Roman Catholic Church. Gregorian chant developed mainly in western and central Europe during the 9th and 10th centuries, with later additions and redactions. Although popular legend credits Pope St. Gregory the Great with inventing Gregorian chant, scholars believe that it arose from a later Carolingian synthesis of Roman chant and Gallican chant." .



###  http://www.semanticweb.org/musicOntology#Guitar

:Guitar rdf:type :Chordophone ,
                 owl:NamedIndividual ;
        
        rdfs:label "Guitar" ;
        
        rdfs:comment "The guitar is a popular musical instrument classified as a string instrument with anywhere from 4 to 18 strings, usually having 6. The sound is projected either acoustically or through electrical amplification (for an acoustic guitar or an electric guitar, respectively). It is typically played by strumming or plucking the strings with the right hand while fretting (or pressing against the fret) the strings with the left hand. The guitar is a type of chordophone, traditionally constructed from wood and strung with either gut, nylon or steel strings and distinguished from other chordophones by its construction and tuning. The modern guitar was preceded by the gittern, the vihuela, the four-course Renaissance guitar, and the five-course baroque guitar, all of which contributed to the development of the modern six-string instrument." .



###  http://www.semanticweb.org/musicOntology#HeavyMetal

:HeavyMetal rdf:type :Rock ,
                     owl:NamedIndividual ;
            
            rdfs:label "Heavy metal" ;
            
            rdfs:comment "Heavy metal (or simply metal) is a genre of rock music that developed in the late 1960s and early 1970s, largely in the United Kingdom and the United States. With roots in blues rock and psychedelic rock, the bands that created heavy metal developed a thick, massive sound, characterized by highly amplified distortion, extended guitar solos, emphatic beats, and overall loudness. Heavy metal lyrics and performance styles are often associated with masculinity, aggression, and machismo." .



###  http://www.semanticweb.org/musicOntology#HerVoiceResides

:HerVoiceResides rdf:type :Song ,
                          owl:NamedIndividual ;
                 
                 rdfs:label "Her Voice Resides" ;
                 
                 :composer :BulletForMyValentine ;
                 
                 :performer :BulletForMyValentine ;
                 
                 :from_album :ThePoison .



###  http://www.semanticweb.org/musicOntology#HighVoltage

:HighVoltage rdf:type :Song ,
                      owl:NamedIndividual ;
             
             rdfs:label "High Voltage" ;
             
             :performer :LinkinPark ;
             
             :composer :LinkinPark .



###  http://www.semanticweb.org/musicOntology#HillCountryBlues

:HillCountryBlues rdf:type :Blues ,
                           owl:NamedIndividual ;
                  
                  rdfs:label "Hill country blues" ;
                  
                  rdfs:comment "Hill Country Blues (also known as The North Mississippi Hill Country Blues or North Mississippi Blues) is a regional style of African American music regarded as distinct from Mississippi Delta blues. It is characterized by a strong emphasis on rhythm and percussion, steady guitar riffs, few chord changes, unconventional song structures, and heavy emphasis on the \"groove\" - more affectionately known as \"the hypnotic boogie.\"" .



###  http://www.semanticweb.org/musicOntology#HipHop

:HipHop rdf:type :Hip-hop ,
                 owl:NamedIndividual .



###  http://www.semanticweb.org/musicOntology#HitTheFloor

:HitTheFloor rdf:type :Song ,
                      owl:NamedIndividual ;
             
             rdfs:label "Hit the Floor" ;
             
             :performer :BulletForMyValentine ;
             
             :composer :BulletForMyValentine ;
             
             :from_album :ThePoison .



###  http://www.semanticweb.org/musicOntology#Hokum

:Hokum rdf:type :Country ,
                owl:NamedIndividual ;
       
       rdfs:label "Hokum" ;
       
       rdfs:comment "Hokum is a particular song type of American blues music—a humorous song which uses extended analogies or euphemistic terms to make sexual innuendos. This trope goes back to early blues recordings, and is seen from time to time in modern American blues and blues rock." .



###  http://www.semanticweb.org/musicOntology#HybridTheory

:HybridTheory rdf:type :Album ,
                       owl:NamedIndividual ;
              
              rdfs:label "Hybrid Theory" ;
              
              :name "Hybrid Theory" ;
              
              rdfs:comment "Hybrid Theory is the debut album by the American rock band Linkin Park, released on October 24, 2000 through Warner Bros. Records. The album was a commercial success, having been certified Diamond for sales of over 10 million units in the United States alone as of 2010, peaking at number two on the Billboard 200, and also reaching high positions on other charts worldwide." ;
              
              :has_song :APlaceForMyHead ,
                        :ByMyself ;
              
              :recorded_on :CD ;
              
              :has_song :Crawling ,
                        :CureForTheItch ;
              
              :recorded_on :DAT ,
                           :DCC ;
              
              :has_song :Forgotten ,
                        :HighVoltage ,
                        :HybridTheory ,
                        :InTheEnd ;
              
              :performer :LinkinPark ;
              
              :recorded_on :MagneticTape ;
              
              :has_song :MyDecember ,
                        :OneStepCloser ,
                        :Papercut ,
                        :PointsOfAuthority ,
                        :PushingMeAway ;
              
              :recorded_on :SACD ;
              
              :has_song :WithYou .



###  http://www.semanticweb.org/musicOntology#Hydraulophone

:Hydraulophone rdf:type :OtherInstruments ,
                        owl:NamedIndividual ;
               
               rdfs:label "Hydraulophone" ;
               
               rdfs:comment "A hydraulophone is a tonal acoustic musical instrument played by direct physical contact with water (sometimes other fluids) where sound is generated or affected hydraulically. Typically sound is produced by the same hydraulic fluid in contact with the player's fingers." .



###  http://www.semanticweb.org/musicOntology#Hymn

:Hymn rdf:type :Religious ,
               owl:NamedIndividual ;
      
      rdfs:label "Hymn" ;
      
      rdfs:comment "A hymn is a type of song, usually religious, specifically written for the purpose of praise, adoration or prayer, and typically addressed to a deity or deities, or to a prominent figure or personification. Although most familiar to speakers of English in the context of Christian churches, hymns are also a fixture of other world religions, especially on the Indian subcontinent. Hymns also survive from antiquity, especially from Egyptian and Greek cultures. Some of the oldest surviving examples of notated music are hymns with Greek texts." .



###  http://www.semanticweb.org/musicOntology#InTheEnd

:InTheEnd rdf:type :Song ,
                   owl:NamedIndividual ;
          
          rdfs:label "In The End" ;
          
          :composer :LinkinPark ;
          
          :performer :LinkinPark .



###  http://www.semanticweb.org/musicOntology#IncredibleMachine

:IncredibleMachine rdf:type :Song ,
                            owl:NamedIndividual ;
                   
                   rdfs:label "Incredible Machine" .



###  http://www.semanticweb.org/musicOntology#InstrumentPlayer

:InstrumentPlayer rdf:type :CollectiveRole ,
                           owl:NamedIndividual ;
                  
                  rdfs:label "Instrument player" .



###  http://www.semanticweb.org/musicOntology#JazzRap

:JazzRap rdf:type :Jazz ,
                  owl:NamedIndividual ;
         
         rdfs:label "Jazz rap" ;
         
         rdfs:comment "Jazz rap is a subgenre of hip hop music that incorporates jazz influences, developed in the late 1980s and early 1990s. The lyrics are often based on political consciousness, Afrocentrism, and general positivism. Allmusic writes that the genre \"was an attempt to fuse African-American music of the past with a newly dominant form of the present, paying tribute to and reinvigorating the former while expanding the horizons of the latter\". Musically, the rhythms have been typically those of hip hop rather than jazz, over which are placed repetitive phrases of jazz instrumentation: trumpet, double bass, etc. The amount of improvisation varies between artists: some groups improvise lyrics and solos, while many of them do not. A Tribe Called Quest, De La Soul and Digable Planets are pioneers of the jazz rap genre." .



###  http://www.semanticweb.org/musicOntology#JenniferNettles

:JenniferNettles rdf:type :Musician ,
                          owl:NamedIndividual ;
                 
                 rdfs:label "Jennifer Nettles" ;
                 
                 rdfs:comment "Jennifer Odessa Nettles (born September 12, 1974) is an American country music artist. She is known primarily for her role as lead vocalist of the duo Sugarland alongside Kristian Bush. Before Sugarland's inception, she also fronted Atlanta-based bands called Soul Miner's Daughter and Jennifer Nettles Band. She also charted as a duet partner on the country version of rock band Bon Jovi's 2006 single \"Who Says You Can't Go Home\", a Number One hit on the Billboard country charts." ;
                 
                 :name "Jennifer Odessa Nettles" ;
                 
                 :plays_on :BassGuitar ,
                           :Guitar ,
                           :Piano ;
                 
                 :primaryMusicalInstrument :Piano .



###  http://www.semanticweb.org/musicOntology#JoeHahn

:JoeHahn rdf:type :Musician ,
                  owl:NamedIndividual ;
         
         rdfs:label "Joe Hahn" ;
         
         :name "Joseph \"Joe\" Hahn" ;
         
         rdfs:comment "Joseph \"Joe\" Hahn (born March 15, 1977), is a turntablist and director best known as the DJ and sampler for the American rock band Linkin Park." ;
         
         :plays_on :Guitar ,
                   :Piano ,
                   :Sampler ;
         
         :primaryMusicalInstrument :Sampler .



###  http://www.semanticweb.org/musicOntology#Kadodi

:Kadodi rdf:type :African ,
                 owl:NamedIndividual ;
        
        rdfs:label "Kadodi" ;
        
        rdfs:comment "is the language spoken by the Kupari community in Vasai, Maharashtra, India. It is also called Samvedic. It may be a divergent dialect of Konkani, with Marathi and Gujarati influence." .



###  http://www.semanticweb.org/musicOntology#Khaliji

:Khaliji rdf:type :Asian ,
                  owl:NamedIndividual ;
         
         rdfs:label "Khaliji" ;
         
         rdfs:comment "Khaliji is a style of music characteristic of Eastern Arabia" .



###  http://www.semanticweb.org/musicOntology#KristianBush

:KristianBush rdf:type :Musician ,
                       owl:NamedIndividual ;
              
              rdfs:label "Kristian Bush" ;
              
              rdfs:comment "Kristian Merrill Bush (born March 14, 1970, in Knoxville, Tennessee, United States) is an American singer, songwriter, producer and multi-instrumentalist. He is best known for being one half of the country music duo Sugarland." ;
              
              :name "Kristian Merrill Bush" ;
              
              :plays_on :ElectricGuitar ;
              
              :primaryMusicalInstrument :Guitar ;
              
              :plays_on :Guitar .



###  http://www.semanticweb.org/musicOntology#LP-BradfordDelson

:LP-BradfordDelson rdf:type :CollectiveMember ,
                            owl:NamedIndividual ;
                   
                   :musician :BradDelson ;
                   
                   :collectiveRole :InstrumentPlayer ,
                                   :Vocal .



###  http://www.semanticweb.org/musicOntology#LP-ChesterBennington

:LP-ChesterBennington rdf:type :CollectiveMember ,
                               owl:NamedIndividual ;
                      
                      :musician :ChesterBennington ;
                      
                      :collectiveRole :Vocal .



###  http://www.semanticweb.org/musicOntology#LP-DaveFarrell

:LP-DaveFarrell rdf:type :CollectiveMember ,
                         owl:NamedIndividual ;
                
                :musician :DaveFarrell ;
                
                :collectiveRole :InstrumentPlayer .



###  http://www.semanticweb.org/musicOntology#LP-JosephHahn

:LP-JosephHahn rdf:type :CollectiveMember ,
                        owl:NamedIndividual ;
               
               :collectiveRole :InstrumentPlayer ;
               
               :musician :JoeHahn ;
               
               :collectiveRole :Vocal .



###  http://www.semanticweb.org/musicOntology#LP-MikeShinoda

:LP-MikeShinoda rdf:type :CollectiveMember ,
                         owl:NamedIndividual ;
                
                :collectiveRole :InstrumentPlayer ;
                
                :musician :MikeShinoda ;
                
                :collectiveRole :Vocal .



###  http://www.semanticweb.org/musicOntology#LP-RobBourdon

:LP-RobBourdon rdf:type :CollectiveMember ,
                        owl:NamedIndividual ;
               
               :collectiveRole :InstrumentPlayer ;
               
               :musician :RobBourdon .



###  http://www.semanticweb.org/musicOntology#LaserHarp

:LaserHarp rdf:type :Electrophone ,
                    owl:NamedIndividual ;
           
           rdfs:label "Laser harp" ;
           
           rdfs:comment "A laser harp is an electronic musical instrument and laser lighting display, consisting of several laser beams to be blocked, in analogy with the plucking of the strings of a harp, in order to produce sounds. The laser harp has been popularized by Jean Michel Jarre, and has been a high profile feature of almost all his concerts since 1981. In recent times, a very similar version has also been used in concerts by British electronic musician Little Boots." .



###  http://www.semanticweb.org/musicOntology#Lavani

:Lavani rdf:type :South-and-southeastAsian ,
                 owl:NamedIndividual ;
        
        rdfs:label "Lavani" ;
        
        rdfs:comment "is a genre of music popular in Maharashtra. Lavani is a combination of traditional song and dance, which particularly performed to the beats of Dholki, a percussion instrument. Lavani is noted for its powerful rhythm. Lavani has contributed substantially to the development of Marathi folk theatre. In Maharashtra and southern Madhya Pradesh, it is performed by the female performers wearing nine-yard long saris. The songs are sung in a quick tempo." .



###  http://www.semanticweb.org/musicOntology#LinkinPark

:LinkinPark rdf:type :Sextet ,
                     owl:NamedIndividual ;
            
            rdfs:label "Linkin Park" ;
            
            :name "Linkin Park" ;
            
            rdfs:comment "Linkin Park is an American rock band from Agoura Hills, California. Formed in 1996, the band rose to international fame with their debut album Hybrid Theory, which was certified Diamond by the RIAA in 2005 and multi-platinum in several other countries. Their following studio album Meteora continued the band's success, topping the Billboard 200 album chart in 2003, and was followed by extensive touring and charity work around the world. In 2003, MTV2 named Linkin Park the sixth-greatest band of the music video era and the third-best of the new millennium. Billboard ranked Linkin Park No. 19 on the Best Artists of the Decade chart. The band was recently voted as the greatest artist of '00s in a Bracket Madness poll on VH1. In 2014, the band was declared as the Biggest Rock Band in the World Right Now by Kerrang." ;
            
            :has_genre :AlternativeRock ;
            
            :has_album :HybridTheory ;
            
            :has_member :LP-BradfordDelson ,
                        :LP-ChesterBennington ,
                        :LP-DaveFarrell ,
                        :LP-JosephHahn ,
                        :LP-MikeShinoda ,
                        :LP-RobBourdon .



###  http://www.semanticweb.org/musicOntology#Liwa

:Liwa rdf:type :Asian ,
               owl:NamedIndividual ;
      
      rdfs:label "Liwa" ;
      
      rdfs:comment "is a traditional dance of African origin performed in Eastern Arabia (Arab states of the Persian Gulf), mainly within communities of descendants of people from the Swahili Coast (Tanzania and Zanzibar). It is also performed by the African-descended Sheedi community, as well as the Baloch of Pakistan's Makran Coast and Karachi area." .



###  http://www.semanticweb.org/musicOntology#LoseYourself

:LoseYourself rdf:type :Song ,
                       owl:NamedIndividual ;
              
              rdfs:label "Lose Yourself" ;
              
              :composer :Eminem ;
              
              :recorded_on :MiniDisc ;
              
              :performer :Solo-Eminem .



###  http://www.semanticweb.org/musicOntology#MagneticTape

:MagneticTape rdf:type :Medium ,
                       owl:NamedIndividual ;
              
              rdfs:label "Magnetic tape" ;
              
              rdfs:comment "Magnetic analogue tape used as medium to record a musical manifestation." .



###  http://www.semanticweb.org/musicOntology#Mambo

:Mambo rdf:type :Latin ,
                owl:NamedIndividual ;
       
       rdfs:label "Mambo" ;
       
       rdfs:comment "Mambo is a musical form and dance style that developed originally in Cuba, with further significant developments by Cuban musicians in Mexico and the USA. The word \"mambo\" means \"conversation with the gods\" in Kikongo, the language spoken by Central African slaves taken to Cuba." .



###  http://www.semanticweb.org/musicOntology#March

:March rdf:type :Occasional ,
                owl:NamedIndividual ;
       
       rdfs:label "March" ;
       
       rdfs:comment "A march, as a musical genre, is a piece of music with a strong regular rhythm which in origin was expressly written for marching to and most frequently performed by a military band. In mood, marches range from the moving death march in Wagner's Götterdämmerung to the brisk military marches of John Philip Sousa and the martial hymns of the late 19th century. Examples of the varied use of the march can be found in Beethoven's Eroica Symphony, in the Marches Militaires of Franz Schubert, in the Marche funèbre in Chopin's Sonata in B flat minor, and in the Dead March in Handel's Saul." .



###  http://www.semanticweb.org/musicOntology#MatthewTuck

:MatthewTuck rdf:type :Musician ,
                      owl:NamedIndividual ;
             
             rdfs:label "Matthew Tuck" ;
             
             :name "Matthew \"Matt\" Tuck" ;
             
             rdfs:comment "Matthew \"Matt\" Tuck (born 20 January 1980) is a Welsh musician. He is the lead vocalist and rhythm guitarist in the Welsh heavy metal band Bullet for My Valentine. He and the other 3 members of his old band founded Jeff Killed John in 1998, but after changing the bassist in 2003, the band was renamed to Bullet for My Valentine.[1] He is also a singer and guitarist in the supergroup AxeWound, which was formed in 2012. He also plays piano, drums, keyboard, and harmonica. He did a collaboration with Max Cavalera of Cavalera Conspiracy and with Apocalyptica in the song \"Repressed\"." ;
             
             :primaryMusicalInstrument :ElectricGuitar ;
             
             :plays_on :ElectricGuitar ,
                       :Guitar ,
                       :Piano .



###  http://www.semanticweb.org/musicOntology#Mellotron

:Mellotron rdf:type :Electrophone ,
                    owl:NamedIndividual ;
           
           rdfs:label "Mellotron" ;
           
           rdfs:comment "The Mellotron is an electro-mechanical, polyphonic tape replay keyboard originally developed and built in Birmingham, England, in 1963. It evolved from a similar instrument, the Chamberlin, but could be mass-produced more effectively. The instrument works by pulling a section of magnetic tape across a head. Different portions of the tape can be played to access different sounds." .



###  http://www.semanticweb.org/musicOntology#MichaelJackson

:MichaelJackson rdf:type :Musician ,
                         owl:NamedIndividual ;
                
                rdfs:label "Michael Jackson" ;
                
                :name "Michael Joseph Jackson" ;
                
                rdfs:comment "Michael Joseph Jackson (August 29, 1958 – June 25, 2009) was an American singer, songwriter, record producer, dancer, and actor. Called the King of Pop, his contributions to music and dance, along with his publicized personal life, made him a global figure in popular culture for over four decades." ;
                
                :plays_on :Drums .



###  http://www.semanticweb.org/musicOntology#MichaelPaget

:MichaelPaget rdf:type :Musician ,
                       owl:NamedIndividual ;
              
              rdfs:label "Michael Paget" ;
              
              :name "Michael Paget" ;
              
              rdfs:comment "Michael Paget (born 12 September 1978), also known as Padge, is a Welsh musician, singer, songwriter, and guitarist. He is the lead guitarist and backing vocalist for the Welsh heavy metal band Bullet for My Valentine." ;
              
              :plays_on :ElectricGuitar ;
              
              :primaryMusicalInstrument :ElectricGuitar .



###  http://www.semanticweb.org/musicOntology#MichaelThomas

:MichaelThomas rdf:type :Musician ,
                        owl:NamedIndividual ;
               
               rdfs:label "Michael Thomas" ;
               
               rdfs:comment """Michael \"Moose\" Thomas (born 4 June 1981) is a Welsh drummer known for his role in heavy metal band Bullet for My Valentine.
Michael Thomas said he first played guitar for two years and then he started playing drums. He said his main influence is Dave Grohl of Nirvana and Foo Fighters and that if it were not for him, he wouldn't be playing drums. Other influences include Scott Travis of Judas Priest, Vinnie Paul of Pantera and Dave Lombardo of Slayer.""" ;
               
               :name "Michael \"Moose\" Thomas" ;
               
               :plays_on :Drums ;
               
               :primaryMusicalInstrument :Drums .



###  http://www.semanticweb.org/musicOntology#MikeShinoda

:MikeShinoda rdf:type :Musician ,
                      owl:NamedIndividual ;
             
             rdfs:label "Mike Shinoda" ;
             
             :name "Michael Kenji \"Mike\" Shinoda" ;
             
             rdfs:comment "Michael Kenji \"Mike\" Shinoda LHD (born February 11, 1977) is an American musician, record producer, and artist. He co-founded Linkin Park in 1996 and is the band's rhythm guitarist, songwriter, keyboardist, and co-vocalist. Shinoda later created a hip hop-driven side project, Fort Minor, in 2003. He served as a producer for tracks and albums by Lupe Fiasco, Styles of Beyond, and The X-Ecutioners." ;
             
             :plays_on :BassGuitar ,
                       :ElectricGuitar ,
                       :Guitar ,
                       :Organ ,
                       :Piano ,
                       :Sampler .



###  http://www.semanticweb.org/musicOntology#MiniDisc

:MiniDisc rdf:type :Medium ,
                   owl:NamedIndividual ;
          
          rdfs:label "Mini Disc" ;
          
          rdfs:comment "Mini Disc used as medium to record a musical manifestation." .



###  http://www.semanticweb.org/musicOntology#Mockingbird

:Mockingbird rdf:type :Song ,
                      owl:NamedIndividual ;
             
             rdfs:label "Mockingbird" ;
             
             :composer :Eminem ;
             
             :recorded_on :MiniDisc ;
             
             :performer :Solo-Eminem .



###  http://www.semanticweb.org/musicOntology#Morlam

:Morlam rdf:type :South-and-southeastAsian ,
                 owl:NamedIndividual ;
        
        rdfs:label "Morlam" ;
        
        rdfs:comment "is a traditional Lao form of song in Laos and Isan. Mor lam means expert song, or expert singer, referring to the music or artist respectively. Other romanisations used include mor lum, maw lam, maw lum, moh lam and mhor lum." .



###  http://www.semanticweb.org/musicOntology#MyDecember

:MyDecember rdf:type :Song ,
                     owl:NamedIndividual ;
            
            rdfs:label "My December" ;
            
            :performer :LinkinPark ;
            
            :composer :LinkinPark .



###  http://www.semanticweb.org/musicOntology#NationalAnthem

:NationalAnthem rdf:type :Occasional ,
                         owl:NamedIndividual ;
                
                rdfs:label "National anthem" ;
                
                rdfs:comment "A national anthem (also national hymn, national song etc.) is a generally patriotic musical composition that evokes and eulogizes the history, traditions and struggles of its people, recognized either by a nation's government as the official national song, or by convention through use by the people. The majority of national anthems are either marches or hymns in style." .



###  http://www.semanticweb.org/musicOntology#Neofolk

:Neofolk rdf:type :Folk ,
                  owl:NamedIndividual ;
         
         rdfs:label "Neofolk" ;
         
         rdfs:comment "Neofolk is a form of folk music-inspired experimental music that emerged from post-industrial music circles. Neofolk can either be solely acoustic folk music or a blend of acoustic folk instrumentation aided by varieties of accompanying sounds such as pianos, strings and elements of industrial music and experimental music. The genre encompasses a wide assortment of themes. Neofolk musicians often have ties to other genres such as neoclassical and martial industrial." .



###  http://www.semanticweb.org/musicOntology#Noise

:Noise rdf:type :Avant-garde ,
                owl:NamedIndividual ;
       
       rdfs:label "Noise" ;
       
       rdfs:comment "Noise music is a category of music that is characterised by the expressive use of noise within a musical context. This type of music tends to challenge the distinction that is made in conventional musical practices between musical and non-musical sound" .



###  http://www.semanticweb.org/musicOntology#NoveltyMusic

:NoveltyMusic rdf:type :Comedy ,
                       owl:NamedIndividual ;
              
              rdfs:label "Novelty music" ;
              
              rdfs:comment "A novelty song is a comical or nonsensical song, performed principally for its comical effect. Humorous songs, or those containing humorous elements, are not necessarily novelty songs. The term arose in Tin Pan Alley to describe one of the major divisions of popular music. The other two divisions were ballads and dance music. Novelty songs achieved great popularity during the 1920s and 1930s." .



###  http://www.semanticweb.org/musicOntology#OneStepCloser

:OneStepCloser rdf:type :Song ,
                        owl:NamedIndividual ;
               
               rdfs:label "One step closer" ;
               
               :performer :LinkinPark ;
               
               :composer :LinkinPark .



###  http://www.semanticweb.org/musicOntology#Onkyokei

:Onkyokei rdf:type :EastAsian ,
                   owl:NamedIndividual ;
          
          rdfs:label "Onkyokei" ;
          
          rdfs:comment "is a form of free improvisation, emerging from Japan in the late 1990s." .



###  http://www.semanticweb.org/musicOntology#Organ

:Organ rdf:type :KeyboardInstrument ,
                owl:NamedIndividual ;
       
       rdfs:label "Organ" ;
       
       rdfs:comment "In music, the organ is a keyboard instrument of one or more divisions, each played with its own keyboard, played either with the hands or with the feet. The organ is a relatively old musical instrument, dating from the time of Ctesibius of Alexandria, who is credited with inventing the water organ. It was played throughout the Greek and Roman world, particularly during races and games. During the early medieval period it spread from the Byzantine Empire, where it continued to be used in secular and imperial court music, to Western Europe, where it gradually assumed a prominent place in the liturgy of the Catholic Church. Subsequently it re-emerged as a secular and recital instrument." .



###  http://www.semanticweb.org/musicOntology#Papercut

:Papercut rdf:type :Song ,
                   owl:NamedIndividual ;
          
          rdfs:label "Papercut" ;
          
          :composer :LinkinPark ;
          
          :performer :LinkinPark .



###  http://www.semanticweb.org/musicOntology#ParodyMusic

:ParodyMusic rdf:type :Comedy ,
                      owl:NamedIndividual ;
             
             rdfs:label "Parody music" ;
             
             rdfs:comment "Parody music, or musical parody, involves changing or copying existing (usually well known) musical ideas or lyrics, or copying the peculiar style of a composer or artist, or even a general style of music. Although the intention of a musical parody may be humour (as in burlesque), it is the re-use of music that is the original defining feature." .



###  http://www.semanticweb.org/musicOntology#Pasodoble

:Pasodoble rdf:type :BallroomDance ,
                    owl:NamedIndividual ;
           
           rdfs:label "Pasodoble" ;
           
           rdfs:comment "Pasodoble, or paso doble, (literal meaning in Spanish: double-step) is a Spanish light music, with a binary rhythm and moderated movement, probably based in typical Spanish dances of XVI century. During the XVIII century it was incorporated to comedies and was adopted as a regulatory step for the Spanish infantry, with a special feature that makes the troops can take the regular step: 120 steps per minute." .



###  http://www.semanticweb.org/musicOntology#Piano

:Piano rdf:type :KeyboardInstrument ,
                owl:NamedIndividual ;
       
       rdfs:label "Piano" ;
       
       rdfs:comment "The piano (an abbreviation of pianoforte) is a musical instrument played using a keyboard. It is widely used in classical and jazz music for solo performances, ensemble use, chamber music, accompaniment, and for composing and rehearsal. Although the piano is not portable and often expensive, its versatility and ubiquity have made it one of the world's most familiar musical instruments." .



###  http://www.semanticweb.org/musicOntology#PointsOfAuthority

:PointsOfAuthority rdf:type :Song ,
                            owl:NamedIndividual ;
                   
                   rdfs:label "Points Of Authority" ;
                   
                   :performer :LinkinPark ;
                   
                   :composer :LinkinPark .



###  http://www.semanticweb.org/musicOntology#Poison

:Poison rdf:type :Song ,
                 owl:NamedIndividual ;
        
        rdfs:label "Poison" ;
        
        :performer :BulletForMyValentine ;
        
        :composer :BulletForMyValentine ;
        
        :from_album :ThePoison .



###  http://www.semanticweb.org/musicOntology#Progressive

:Progressive rdf:type :Electronic ,
                      owl:NamedIndividual ;
             
             rdfs:label "Progressive house" ;
             
             rdfs:comment "Progressive house is a style (subgenre) of house music. The progressive house style emerged in the early 1990s. It initially developed in the United Kingdom as a natural progression of American and European house music of the late 1980s. The genre was heavily influenced by trance in the 1990s and later by big room house and Eurodance in the mid-2000s. As of November 2014, the genre is rated first in a list of top genres at TopDeejays." .



###  http://www.semanticweb.org/musicOntology#ProgressiveRock

:ProgressiveRock rdf:type :Rock ,
                          owl:NamedIndividual ;
                 
                 rdfs:label "Progressive rock" ;
                 
                 rdfs:comment "Progressive rock, also known as prog rock or prog, is a rock music subgenre that originated in the United Kingdom with further developments in Germany, Italy, and France, throughout the mid-to-late 1960s and 1970s. It developed from psychedelic rock, and originated, similarly to art rock, as an attempt to give greater artistic weight and credibility to rock music. Bands abandoned the short pop single in favor of instrumentation and compositional techniques more frequently associated with jazz or classical music in an effort to give rock music the same level of musical sophistication and critical respect." .



###  http://www.semanticweb.org/musicOntology#Punta

:Punta rdf:type :Caribbean-and-Caribbean-influenced ,
                owl:NamedIndividual ;
       
       rdfs:label "Punta" ;
       
       rdfs:comment "Punta is a Garifuna music and dance style performed at celebrations and festive occasions. A dance and music created by the Garifuna people of present day St. Vincent and Dominica." .



###  http://www.semanticweb.org/musicOntology#PushingMeAway

:PushingMeAway rdf:type :Song ,
                        owl:NamedIndividual ;
               
               rdfs:label "Pushing Me Away" ;
               
               :composer :LinkinPark ;
               
               :performer :LinkinPark .



###  http://www.semanticweb.org/musicOntology#Pyrophone

:Pyrophone rdf:type :OtherInstruments ,
                    owl:NamedIndividual ;
           
           rdfs:label "Pyrophone" ;
           
           rdfs:comment "A pyrophone, also known as a \"fire/explosion organ\" or \"fire/explosion calliope\" is a musical instrument in which notes are sounded by explosions, or similar forms of rapid combustion, rapid heating, or the like. It was invented by Georges Frédéric Eugène Kastner." .



###  http://www.semanticweb.org/musicOntology#Ragga

:Ragga rdf:type :Hip-hop ,
                owl:NamedIndividual ;
       
       rdfs:label "Ragga" ;
       
       rdfs:comment "Raggamuffin music, usually abbreviated as ragga, is a subgenre of dancehall music or reggae, in which the instrumentation primarily consists of electronic music. Similar to hip hop, sampling often serves a prominent role in raggamuffin music." .



###  http://www.semanticweb.org/musicOntology#Rasin

:Rasin rdf:type :Caribbean-and-Caribbean-influenced ,
                owl:NamedIndividual ;
       
       rdfs:label "Rasin" ;
       
       rdfs:comment "Rasin is a musical style that began in Haïti in the 1970s when musicians began combining elements of traditional Haïtian Vodou ceremonial and folkloric music with rock and roll. This style of modern music reaching back to the roots of Vodou tradition came to be called mizik rasin (\"roots music\") in Haitian Creole or musique racine in French. In context, the movement is often referred to simply as rasin or racine." .



###  http://www.semanticweb.org/musicOntology#RobBourdon

:RobBourdon rdf:type :Musician ,
                     owl:NamedIndividual ;
            
            rdfs:label "Rob Bourdon" ;
            
            rdfs:comment "Robert Gregory Bourdon (born January 20, 1979) is the drummer and youngest member of the rock band Linkin Park." ;
            
            :name "Robert Gregory Bourdon" ;
            
            :plays_on :Drums ;
            
            :primaryMusicalInstrument :Drums .



###  http://www.semanticweb.org/musicOntology#Room409

:Room409 rdf:type :Song ,
                  owl:NamedIndividual ;
         
         rdfs:label "Room 409" ;
         
         :composer :BulletForMyValentine ;
         
         :performer :BulletForMyValentine ;
         
         :from_album :ThePoison .



###  http://www.semanticweb.org/musicOntology#Runaway

:Runaway rdf:type :Song ,
                  owl:NamedIndividual ;
         
         rdfs:label "Runaway" ;
         
         :performer :LinkinPark ;
         
         :composer :LinkinPark .



###  http://www.semanticweb.org/musicOntology#SACD

:SACD rdf:type :Medium ,
               owl:NamedIndividual ;
      
      rdfs:label "Super Audio Compact Disc" ;
      
      rdfs:comment "Super Audio Compact Disc used as medium to record a musical manifestation." .



###  http://www.semanticweb.org/musicOntology#Samba

:Samba rdf:type :Brazilian ,
                owl:NamedIndividual ;
       
       rdfs:label "Samba" ;
       
       rdfs:comment "Samba is a Brazilian musical genre and dance style originating in Brazil, with its roots in Africa via the West African slave trade and African religious traditions, particularly Angola and the Congo. Although there were various forms of samba in Brazil in the form of various popular rhythms and regional dances that originated from the drumming, samba as music genre is seen as a musical expression of urban Rio de Janeiro, then the capital of Imperial Brazil." .



###  http://www.semanticweb.org/musicOntology#Sampler

:Sampler rdf:type :Electrophone ,
                  owl:NamedIndividual ;
         
         rdfs:label "Sampler" ;
         
         rdfs:comment "A sampler (or, in the case of only playback, called sample player or Rompler) is an electronic musical instrument similar in some respects to a synthesizer but, instead of generating sounds, it uses recordings (or \"samples\") of sounds that are loaded or recorded into it by the user and then played back by means of the sampler program itself, a keyboard, sequencer or other triggering device to perform or compose music. Because these samples are now usually stored in digital memory the information can be quickly accessed. A single sample may often be pitch-shifted to produce musical scales and chords." .



###  http://www.semanticweb.org/musicOntology#Sawt

:Sawt rdf:type :Asian ,
               owl:NamedIndividual ;
      
      rdfs:label "Sawt" ;
      
      rdfs:comment "is a kind of popular music found in Kuwait and Bahrain. Sawt is a complex form of urban music, originally performed by 'ud (plucked lute) and mirwas (a drum), with a violin later supplementing the arrangement." .



###  http://www.semanticweb.org/musicOntology#Solo-AndreaBocelli

:Solo-AndreaBocelli rdf:type :SoloPerformer ,
                             owl:NamedIndividual ;
                    
                    :has_genre :AdultContemporary .



###  http://www.semanticweb.org/musicOntology#Solo-Eminem

:Solo-Eminem rdf:type :SoloPerformer ,
                      owl:NamedIndividual ;
             
             :musician :Eminem ;
             
             :has_genre :HipHop .



###  http://www.semanticweb.org/musicOntology#Solo-MichaelJackson

:Solo-MichaelJackson rdf:type :SoloPerformer ,
                              owl:NamedIndividual ;
                     
                     :has_genre :Dance-pop ;
                     
                     :musician :MichaelJackson .



###  http://www.semanticweb.org/musicOntology#Spiritual

:Spiritual rdf:type :Religious ,
                    owl:NamedIndividual ;
           
           rdfs:label "Spiritual" ;
           
           rdfs:comment "Spirituals (or Negro spirituals) are religious (generally Christian) songs that were created by enslaved African people in the United States. Although spirituals were originally unaccompanied monophonic (unison) songs, they are best known today in harmonized choral arrangements." .



###  http://www.semanticweb.org/musicOntology#StandUp

:StandUp rdf:type :Song ,
                  owl:NamedIndividual ;
         
         rdfs:label "Stand Up" .



###  http://www.semanticweb.org/musicOntology#StuckLikeGlue

:StuckLikeGlue rdf:type :Song ,
                        owl:NamedIndividual ;
               
               rdfs:label "Stuck Like Glue" .



###  http://www.semanticweb.org/musicOntology#SuffocatingUnderWordsOfSorrow

:SuffocatingUnderWordsOfSorrow rdf:type :Song ,
                                        owl:NamedIndividual ;
                               
                               rdfs:label "Suffocating Under Words of Sorrow" ;
                               
                               :composer :BulletForMyValentine ;
                               
                               :performer :BulletForMyValentine ;
                               
                               :from_album :ThePoison .



###  http://www.semanticweb.org/musicOntology#Sugarland

:Sugarland rdf:type :Duet ,
                    owl:NamedIndividual ;
           
           rdfs:label "Sugarland" ;
           
           rdfs:comment "Sugarland, an American country music duo, is composed of singer–songwriters Jennifer Nettles (lead vocals) and Kristian Bush (background vocals, lead vocals, mandolin, acoustic guitar, and harmonica). Sugarland was founded in 2002 by Kristen Hall with Bush and ultimately became a trio after hiring Jennifer Nettles as lead singer. After three years, Hall left the group." ;
           
           :composer_of :AllWeAre ;
           
           :performs :AllWeAre ,
                     :EveryGirlLikeMe ;
           
           :composer_of :EveryGirlLikeMe ;
           
           :performs :IncredibleMachine ;
           
           :composer_of :IncredibleMachine ,
                        :StandUp ;
           
           :performs :StandUp ;
           
           :composer_of :StuckLikeGlue ;
           
           :performs :StuckLikeGlue ;
           
           :has_member :Sugarland-JenniferNettles ,
                       :Sugarland-KristianBush ;
           
           :has_genre :TexasCountry ;
           
           :has_album :TheIncredibleMachine ;
           
           :performs :Tonight ;
           
           :composer_of :Tonight .



###  http://www.semanticweb.org/musicOntology#Sugarland-JenniferNettles

:Sugarland-JenniferNettles rdf:type :CollectiveMember ,
                                    owl:NamedIndividual ;
                           
                           :collectiveRole :InstrumentPlayer ;
                           
                           :musician :JenniferNettles ;
                           
                           :collectiveRole :Vocal .



###  http://www.semanticweb.org/musicOntology#Sugarland-KristianBush

:Sugarland-KristianBush rdf:type :CollectiveMember ,
                                 owl:NamedIndividual ;
                        
                        :collectiveRole :InstrumentPlayer ;
                        
                        :musician :KristianBush ;
                        
                        :collectiveRole :Vocal .



###  http://www.semanticweb.org/musicOntology#Tango

:Tango rdf:type :BallroomDance ,
                owl:NamedIndividual ;
       
       rdfs:label "Tango" ;
       
       rdfs:comment "Tango is a style of music in 2/4 or 4/4 time that originated among European immigrant populations of Argentina and Uruguay (collectively, the \"Rioplatenses\")." .



###  http://www.semanticweb.org/musicOntology#TearsDontFall

:TearsDontFall rdf:type :Song ,
                        owl:NamedIndividual ;
               
               rdfs:label "Tears Dont Fall" ;
               
               :composer :BulletForMyValentine ;
               
               :performer :BulletForMyValentine ;
               
               :from_album :ThePoison .



###  http://www.semanticweb.org/musicOntology#Techno

:Techno rdf:type :Electronic ,
                 owl:NamedIndividual ;
        
        rdfs:label "Techno" ;
        
        rdfs:comment "Techno is a form of electronic dance music that emerged in Detroit, Michigan, in the United States during the mid-to-late 1980s. The first recorded use of the word techno in reference to a specific genre of music was in 1988. Many styles of techno now exist, but Detroit techno is seen as the foundation upon which a number of subgenres have been built." .



###  http://www.semanticweb.org/musicOntology#TexasCountry

:TexasCountry rdf:type :Country ,
                       owl:NamedIndividual ;
              
              rdfs:label "Texas country" ;
              
              rdfs:comment "Texas country music (more popularly known just as Texas country or Texas music) is a rapidly growing subgenre of American country music. Texas country is known for fusing traditionalist root sounds (similar to neotraditional country) with the outspoken, care-free views of outlaw country. Texas country blends these subgenres by featuring straightforward, truthful lyrics, a \"take it or leave it\" approach, a \"common working man\" theme, comical, witty undertones, intense live performances, and loyal fan-bases. These often combine with stripped down music, increasing the intimate connection between a singer and audience. Texas Country Music can also be called, \"Red Dirt\" country music, which originated in Oklahoma. The two states, Texas and Oklahoma, have influenced the scene of this particular genre. Both states have fled the scene of recent main-stream country music, to create their own respective sound." .



###  http://www.semanticweb.org/musicOntology#TheIncredibleMachine

:TheIncredibleMachine rdf:type :Album ,
                               owl:NamedIndividual ;
                      
                      rdfs:label "The Incredible Machine" ;
                      
                      rdfs:comment "The Incredible Machine is the fourth studio album by American country music duo Sugarland. It was released on October 19, 2010 via Mercury Nashville Records. Byron Gallimore along with both members Jennifer Nettles and Kristian Bush teamed up for production of the album." ;
                      
                      :has_song :AllWeAre ;
                      
                      :recorded_on :CD ,
                                   :DAT ,
                                   :DCC ;
                      
                      :has_song :EveryGirlLikeMe ,
                                :IncredibleMachine ,
                                :StandUp ,
                                :StuckLikeGlue ;
                      
                      :performer :Sugarland ;
                      
                      :has_song :Tonight .



###  http://www.semanticweb.org/musicOntology#ThePoison

:ThePoison rdf:type :Album ,
                    owl:NamedIndividual ;
           
           rdfs:label "The Poison" ;
           
           rdfs:comment "The Poison is the debut album by Welsh heavy metal band Bullet for My Valentine. The album was released on 3 October 2005 through Visible Noise Records in the UK, and on February 14, 2006 in the United States through Trustkill Records. The album included 11 new songs and two previously heard songs, \"Cries in Vain\", which was previously heard from their self-titled UK EP and from their US EP, Hand of Blood, as well as from \"4 Words (To Choke Upon)\" was previously included on the same US release. Different editions of the album contain the song \"Hand of Blood\", previously heard from these EPs, replacing \"Spit You Out\"." ;
           
           :performer :BulletForMyValentine ;
           
           :recorded_on :CD ,
                        :DAT ,
                        :DCC ,
                        :DVD-Audio ,
                        :MagneticTape ,
                        :MiniDisc ,
                        :Vinyl .



###  http://www.semanticweb.org/musicOntology#Tonbak

:Tonbak rdf:type :Membranophone ,
                 owl:NamedIndividual ;
        
        rdfs:label "Tonbak" ;
        
        rdfs:comment "The Tompak (official Persian name), also tombak, donbak, dombak or zarb is a goblet drum from Persia (ancient Iran). It is considered the principal percussion instrument of Persian music. The tonbak is normally positioned diagonally across the torso while the player uses one or more fingers and/or the palm(s) of the hand(s) on the drumhead, often (for a ringing timbre) near the drumhead's edge. Sometimes tonbak players wear metal finger rings for an extra-percussive \"click\" on the drum's shell. Tonbak virtuosi perform solos lasting ten minutes or more." .



###  http://www.semanticweb.org/musicOntology#Tonight

:Tonight rdf:type :Song ,
                  owl:NamedIndividual ;
         
         rdfs:label "Tonight" .



###  http://www.semanticweb.org/musicOntology#Trance

:Trance rdf:type :Electronic ,
                 owl:NamedIndividual ;
        
        rdfs:label "Trance" ;
        
        rdfs:comment "Trance is a genre of electronic dance music that developed in the 1990s in Germany. It is characterized by a tempo of between 125 to mid 140 beats per minute (BPM), repeating melodic phrases, and a musical form that distinctly builds up and down throughout a track. Although trance is a genre of its own, it liberally incorporates influences from other electronic music styles such as techno, house, pop, chill-out, classical music, and film music." .



###  http://www.semanticweb.org/musicOntology#Triangle

:Triangle rdf:type :Idiophone ,
                   owl:NamedIndividual ;
          
          rdfs:label "Triangle" ;
          
          rdfs:comment "The triangle is an idiophone type of musical instrument in the percussion family. It is a bar of metal, usually steel but sometimes other metals like beryllium copper, bent into a triangle shape. The instrument is usually held by a loop of some form of thread or wire at the top curve. It was first made around the 16th century." .



###  http://www.semanticweb.org/musicOntology#Trumpet

:Trumpet rdf:type :Aerophone ,
                  owl:NamedIndividual ;
         
         rdfs:label "Trumpet" ;
         
         rdfs:comment "A trumpet is a musical instrument. It is the highest register in the brass family. Trumpets are among the oldest musical instruments, dating back to at least 1500 BC. They are played by blowing air through closed lips, producing a \"buzzing\" sound that starts a standing wave vibration in the air column inside the instrument. Since the late 15th century they have primarily been constructed of brass tubing, usually bent twice into a rounded oblong shape." .



###  http://www.semanticweb.org/musicOntology#Vinyl

:Vinyl rdf:type :Medium ,
                owl:NamedIndividual ;
       
       rdfs:label "Vinyl" ;
       
       rdfs:comment "Vinyl used as medium to record a musical manifestation" .



###  http://www.semanticweb.org/musicOntology#Violin

:Violin rdf:type :Chordophone ,
                 owl:NamedIndividual ;
        
        rdfs:label "Violin" ;
        
        rdfs:comment "The violin, also known as a fiddle, is a string instrument, usually with four strings tuned in perfect fifths. It is the smallest, highest-pitched member of the violin family of string instruments, which also includes the viola, and the cello. The modern word is derived from the Italian word violino, literally 'small viola'." .



###  http://www.semanticweb.org/musicOntology#Vocal

:Vocal rdf:type :CollectiveRole ,
                owl:NamedIndividual ;
       
       rdfs:label "Vocal" .



###  http://www.semanticweb.org/musicOntology#WithYou

:WithYou rdf:type :Song ,
                  owl:NamedIndividual ;
         
         rdfs:label "With You" ;
         
         :performer :LinkinPark ;
         
         :composer :LinkinPark .



###  http://www.semanticweb.org/musicOntology#WrongOfMe

:WrongOfMe rdf:type :Song ,
                    owl:NamedIndividual ;
           
           rdfs:label "Wrong of Me" ;
           
           :composer :BulletForMyValentine ;
           
           :performer :BulletForMyValentine .



###  http://www.semanticweb.org/musicOntology#Xylophone

:Xylophone rdf:type :Idiophone ,
                    owl:NamedIndividual ;
           
           rdfs:label "Xylophone" ;
           
           rdfs:comment "The xylophone is a musical instrument in the percussion family that consists of wooden bars struck by mallets. Each bar is an idiophone tuned to a pitch of a musical scale, whether pentatonic or heptatonic in the case of many African and Asian instruments, diatonic in many western children's instruments, or chromatic for orchestral use." .



###  http://www.semanticweb.org/musicOntology#Zydeco

:Zydeco rdf:type :Country ,
                 owl:NamedIndividual ;
        
        rdfs:label "Zydeco" ;
        
        rdfs:comment "Zydeco is a musical genre evolved in southwest Louisiana by French Creole speakers which blends blues, rhythm and blues, and music indigenous to the Louisiana Creoles and the Native people of Louisiana." .





#################################################################
#
#    General axioms
#
#################################################################


[ rdf:type owl:AllDisjointClasses ;
  owl:members ( :Aerophone
                :Chordophone
                :Electrophone
                :KeyboardInstrument
                :OtherInstruments
                :Percussion
              )
] .
[ rdf:type owl:AllDisjointClasses ;
  owl:members ( :Duet
                :Ensemble
                :Octet
                :Quartet
                :Quintet
                :Septet
                :Sextet
                :Trio
              )
] .




###  Generated by the OWL API (version 3.4.2) http://owlapi.sourceforge.net

